# Integrals and Cauchy's Theorem

## 9

- Note $f$ is continuous on $\CC$ since analytic implies continuous ($f$ equals its power series, where the partials sums uniformly converge to it, and uniform limit of continuous is continuous).
- Strategy: take $D$ a disc centered at a point $x\in \RR$, show $f$ is holomorphic in $D$ by Morera's theorem.
- Let $\Delta \subset D$ be a triangle in $D$.
- Case 1: If $\Delta \intersect \RR = 0$, then $f$ is holomorphic on $\Delta$ and $\int_\Delta f = 0$.
- Case 2: one side or vertex of $\Delta$ intersects $\RR$, and wlog the rest of $\Delta$ is in $\HH^+$.
  - Then let $\Delta_\eps$ be the perturbation $\Delta + i\eps = \theset{z+ i\eps \suchthat z\in \Delta}$; then $\Delta_\eps \intersect \RR = 0$ and $\int_{\Delta_\eps} f = 0$.
  - Now let $\eps\to 0$ and conclude by continuity of $f$ (???)
    - We want
    \begin{align*}
    \int_{\Delta_\eps} f = \int_a^b f(\gamma_\eps(t)) \gamma_\eps'(t)\,dt \converges{\eps\to 0}\to \int_a^b f(\gamma(t)) \gamma_\eps'(t)\,dt =\int_{\Delta}  f
    \end{align*}
    where $\gamma_\eps, \gamma$ are curves parametrizing $\Delta_\eps, \Delta$ respectively.
    - Since $\gamma, \gamma_\eps$ are closed and bounded in $\CC$, they are compact subsets. Thus it suffices to show that $f(\gamma_\eps(t)) \gamma_\eps'(t)$ converges uniformly to $f(\gamma(t))\gamma'(t)$.
    -  ??
- Case 3: $\Delta$ intersects both $\HH^+$ and $\HH^-$.
  - Break into smaller triangles, each of which falls into one of the previous two cases.

# Laurent Polynomials

## 1

Let $f(z) = {z+1\over z(z-1)}$.

About $z=0$:

\begin{align*}
f(z) 
&= (z+1) \qty{- {1 \over z} + {1\over z-1} } \\
&=  -(z+1) \qty{{1\over z} + \sum_{n=0}^\infty z^n } \\
&= -(z+1)\sum_{n=-1}^\infty z^n \\
&= {1\over z} + 2\sum_{n=0}^\infty z^n \\
&= -{1\over z} -2 - 2z - 2z^2 - \cdots
.\end{align*}

About $z=1$:

\begin{align*}
f(z) 
&= \qty{(1-z) -2 \over 1-z} \qty{1 \over 1 - (1-z)} \\
&= \qty{1 - {2\over 1-z}} \sum_{n=0}^\infty (1-z)^n \\ 
&= \sum_{n=0}^\infty (1-z)^n - 2 \sum_{n=-1}^\infty (1-z)^n \\
&= -{2\over 1-z} - \sum_{n=0}^\infty (1-z)^n \\
&= {2\over z-1} + \sum_{n=0}^\infty (-1)^{n+1} (z-1)^n \\
&= {2\over z-1} - 1 + (z-1) - (z-1)^2 + \cdots
.\end{align*}


## 2

\begin{align*}
e^{1\over z} = \sum_{n=0}^\infty {1\over n!} \qty{1\over z}^n = 1 + {1\over z} + {1 \over 2z^2} + {1\over 6z^3} + \cdots
.\end{align*}

\begin{align*}
\cos\qty{1\over z} 
&= {1\over 2}\qty{ e^{i\over z} + e^{-{i\over z}} }  \\
&= {1\over 2} \sum_{n=0}^\infty {1\over n!}\qty{ \qty{i\over z}^n + \qty{-i \over z}^n  } \\
&= \sum_{n=0}^\infty {(-1)^n \over (2n)!} \qty{1\over z}^{2n}
.\end{align*}
