---
title: 'Section 8.6: The Solutions of the Floer Equation are "Somewhere Injective".'
---

[Floer Reading Group Fall 2020](../../../../zets/Floer%20Reading%20Group%20Fall%202020.md)

Tags: #floer #topology 

## Outline

Two Goals:

1. Critical points are discrete and regular points are open/dense.
2. The continuation principle (used elsewhere, see diagram later) 
  - Idea: For $\CC$, a holomorphic function with all derivatives vanishing on a line is identically zero.


## Outline of Statements

\begin{center}
\includegraphics[width = 0.4\textwidth]{figures/image_2020-05-11-00-55-25.png} 
\end{center}

\begin{center}
\includegraphics[width = \textwidth]{figures/image_2020-05-13-18-45-19.png} 
\end{center}

What we'll try to prove:

- 8.6.1: Reduction to Cauchy-Riemann equations on $\RR^2$ (short)
- 8.6.3 (Partial): $R(v)$ is open.

\newpage 

Statements of "big" theorems for the chapter, in reverse order of implication:

- 8.1.5: $(d\mcf)_u$ is a Fredholm operator of index $\mu(x) - \mu(y)$.
- 8.1.4: $\Gamma: W^{1, p} \cross C_\eps^\infty \to L^p$ has a continuous right-inverse and is surjective
- 8.1.3: $\mcz(x, y, J)$ is a Banach manifold
- 8.1.1: For $h\in \mch_{\text{reg}}, H_0 + h$ is nondegenerate and $(d\mcf)_u$ is surjective for every $u\in \mcm(H_0 + h, J)$.
- 8.1.2: For $h \in \mch_{\text{reg}}$ and all contractible orbits $x, y$ of $H_0$, $\mcm(x, y, H_0 + h)$ is a manifold of dimension $\mu(x) - \mu(y)$.

## Notation

- The Floer equation and its linearization:
\begin{align*}
\mcf(u) &= \dd{u}{s} + J \dd{u}{t} + \grad_u(H) = 0 \\
\qty{d\mcf}_u(Y) &= \dd{Y}{s} + J_0 \dd{Y}{t} + S\cdot Y \\ 
&Y\in u^* TW,~ S \in C^\infty(\RR\cross S^1; \endo(\RR^{2n}))
.\end{align*}

- $X(t, u): S^1\cross W \to W$ is a time-dependent periodic vector field on $\RR^{2n}$, $J$ an almost-complex structure, both smooth

- $u \in C^\infty(\RR \cross S^1; W)$ is a solution to the equation 
$$\dd{u}{s} + J(t, u) \qty{\dd{u}{t} - X(t, u)} = 0$$

  > Note: not sure why we've replaced $\grad_u(H)$ with $-J(t, u) \cdot X(t, u)$ in the Floer equation.

- $C(u)$ the set of critical points and $R(u)$ the set of regular points of $u$:
\begin{align*}
(s_0, t_0) \in C(u) \subseteq \RR\cross S^1 &\iff \dd{u}{s}(s_0, t_0) = 0 \\
(s_0, t_0) \in R(u) \subset \RR \cross S^1 &\iff (s_0, t_0) \not\in C(u)  ~\& ~s\neq s_0 \implies u(s_0, t_0) \neq u(s, t_0)
.\end{align*}

\newpage 

## Goal 1: Discrete Critical Points and Dense Regular Points

Goal 1: prove the following theorem

Theorem (8.5.4)
:   \hfill

    1. $C(u)$ is discrete and 
    2. $R(u) \injects \RR \cross S^1$ is open and dense.

Outline of the proof:
\normalsize

- Prove 8.6.1: Reduction to CR 
  - (direct, short) which transforms the Floer(?) equation
    $$\dd{u}{s} + J(t, u) \qty{\dd{u}{t} - X(t, u)} = 0 \qtext{where} u \in C^\infty(\RR\cross S^1; W)$$
    to a Cauchy-Riemann equation on $\RR^2$:
    $$\dd{v}{s} + J \dd{v}{t} = 0 \qtext{where} v\in C^\infty(\RR^2; W)$$
- Reduce 8.5.4 (Discrete/Open/Dense) to two statements
  - 8.6.2: $C(v)$ (and thus $C(u)$) is discrete
    Proved later using 8.6.8: *Similarity Principle*.
  - 8.6.3 (Injectivity): 
    If $v$ is a smooth periodic solution of CR with $\dd{v}{s}\neq 0$ then $R(v) \subseteq \RR^2$ is open and dense.
- Prove 8.6.3 (Injectivity)
  - Show open (easier)
  - Show dense (delicate!)
- Prove 8.6.8: Similarity Principle
  - Use similarity principle to prove 8.6.6: Continuation Principle. Yields theorem.

\begin{center}
\includegraphics[width = 0.8\textwidth]{figures/image_2020-05-13-18-45-19.png} 
\end{center}

\newpage

\large
<!--digraph {-->
 <!--compound=true-->
<!--subgraph cluster_1 {-->
  <!--"8.5.4: C(u) discrete and R(u) open/dense" [shape=oval fillcolor="cyan" style=filled]-->
  <!--"8.6.2: C(v) discrete" -> "8.5.4: C(u) discrete and R(u) open/dense"-->
  <!--"8.6.3: R(v) open/dense ('Injectivity')" -> "8.5.4: C(u) discrete and R(u) open/dense"-->
<!--}-->

<!--subgraph cluster_2 {-->
  <!--"8.1.1: Nondegenerate Perturbations and Surjective Differential" [shape=box]-->
  <!--"8.1.2: Trajectories x->y Form a Manifold of the Right Dimension" [shape=box]-->
  <!--"8.1.3: Z(x,y,J) is a Banach Manifold" [shape=box]-->
  <!--"8.1.4: Gamma is Surjective" [shape=box]-->
  <!--"8.1.5: dF is Fredholm" [shape=box]-->
  <!--"8.5.4: Sard-Smale" -> "8.1.1: Nondegenerate Perturbations and Surjective Differential"-->

<!--}-->

<!--"8.1.1: Nondegenerate Perturbations and Surjective Differential" -> "8.1.2: Trajectories x->y Form a Manifold of the Right Dimension"-->
<!--"8.1.3: Z(x,y,J) is a Banach Manifold" -> "8.1.1: Nondegenerate Perturbations and Surjective Differential" -->
<!--"8.1.4: Gamma is Surjective" [shape=box]-->
<!--"8.1.4: Gamma is Surjective" -> "8.1.3: Z(x,y,J) is a Banach Manifold"-->
<!--"8.1.5: dF is Fredholm" -> "8.1.4: Gamma is Surjective"-->
<!--"8.6.5: Unique v Solutions in a Small Ball" -> "8.6.4: Failure of Injectivity"-->
<!--"8.6.4: Failure of Injectivity" -> "8.6.3: R(v) open/dense ('Injectivity')"-->

<!--subgraph cluster_3 {-->
<!--"8.6.8: Similarity Principle"-->
<!--"8.6.11: del bar is surjective Fredholm" [shape=box]-->
<!--"8.6.10: Existence of a Nice Operator A"-->
<!--"8.6.11: del bar is surjective Fredholm" -> "8.6.10: Existence of a Nice Operator A"-->
<!--"8.6.10: Existence of a Nice Operator A" -> "8.6.8: Similarity Principle"-->
<!--}-->

<!--"8.6.6: Continuation Principle" [shape=oval fillcolor="cyan" style=filled]-->
<!--"8.6.8: Similarity Principle" -> "8.6.2: C(v) discrete"-->
<!--"8.6.8: Similarity Principle" -> "8.6.6: Continuation Principle"-->
<!--"8.6.1: Reduction to CR on R2" -> "8.6.2: C(v) discrete" [lhead=cluster_1]-->
<!--"8.6.6: Continuation Principle" -> "8.6.5: Unique v Solutions in a Small Ball"-->
<!--"8.6.6: Continuation Principle" -> "8.1.4: Gamma is Surjective"-->
<!--"8.5.4: C(u) discrete and R(u) open/dense" -> "8.1.1: Nondegenerate Perturbations and Surjective Differential"-->
<!--}-->



## 8.6.1: Transform to Cauchy-Riemann

Proposition (8.6.1, Transform to CR-equation on R2)
:   If $u$ is a solution to the following equation:
    \begin{align*}
    \frac{\partial u}{\partial s}+J(t, u)\left(\frac{\partial u}{\partial t}-X(t, u)\right)=0
    .\end{align*}

    Then there exists

    - An almost complex structure $J_1$
    - A diffeomorphism $\varphi$ on $W$ ?
    - A map $v \in C^\infty(\RR^2; W)$

    satisfying

    $$
      \dd{v}{s} + J_1(v) \dd{v}{t} = 0 
    $$

    where
    
    1. $v(s, t+1) = \varphi(v(s, t))$
    
    2. $C(u) = C(v)$, i.e. $u, v$ have the same critical points
    
    3. $R(u) = R(v)$.



Proof

- Recall the vector field was defined as $X(t, u): S^1\cross W \to W$.

- Since $W\cross S^1$ is compact, the flow $\psi_t$ of $X_t$ is defined on all of $W$
  - We thus have a map $\psi_t: W\to W$ such that
$$\dd{}{t}\psi_t = X_t \circ \psi_t, \quad\quad \psi_0 = \id$$


- Define the (important!) map 
  $$v(s, t) \definedas \qty{\psi_t\inv \circ u}(s, t)$$

\newpage

- Since $W\cross S^1$ is compact, the flow $\psi_t$ of $X_t$ is defined on all of $W$
  - We thus have a map $\psi_t: W\to W$ such that
$$\dd{}{t}\psi_t = X_t \circ \psi_t, \quad\quad \psi_0 = \id$$

- Define the (important!) map 
  $$v(s, t) \definedas \qty{\psi_t\inv \circ u}(s, t)$$

- We can then compute
\begin{align*}
\dd{u}{s} &= \color{blue} \qty{d\psi_t} \qty{\dd{v}{s}}  \\
\dd{u}{t} &= \color{orange} \qty{d\psi_t} \qty{\dd{v}{t}} + X_t(u)
.\end{align*}

  - Attempt at explanation: rearrange, use chain rule, and known derivative of $\psi_t$:
  \begin{align*}
  u(s, t) = \qty{\psi_t \circ v}(s, t) 
&\implies \dd{u}{s}(s, t) = \dd{\psi_t}{s}\qty{v(s, t)} \cdot \dd{v}{s}(s, t) \\ \\
{}_? &\implies \dd{u}{s} = \qty{d \psi_t} \cdot \qty{\dd{v}{s}}
  \end{align*}
  and
  \begin{align*}
\dd{u}{t}(s, t) &= \dd{\psi_t}{t}\qty{v(s, t)} \cdot \dd{v}{t}(s, t) \\
  &= \qty{X_t \circ \psi_t}(v(s, t)) \cdot \dd{v}{t}{(s, t)} \\
  &= \qty{X_t \circ \color{red}\psi_t\circ v}(s, t) \cdot \dd{v}{t}{(s, t)} \\
  &= X_t(u(s, t))  \cdot \dd{v}{t}{(s, t)} \\
  &= X_t(u) \qty{\dd{v}{t}} \cdots ????
  .\end{align*}

> Note sure how to relate partial derivatives $\dd{}{\wait} \psi_t$ to differential $d\psi_t$.
> Not sure why we're picking up *addition* in the $t$ derivative.

\newpage

- Given that result, we can compute,
\begin{align*}
0 
&= \frac{\partial u}{\partial s}+J\left(\frac{\partial u}{\partial t}-X_{t}(u)\right) &\text{since $u$ is a solution} \\
&= {\color{blue} \dd{u}{s}} + J {\color{orange} \dd{u}{t}} - J X_t(u) &\text{expanding terms} \\
&= \qty{\color{blue} \qty{d\psi_t} \qty{\dd{v}{s}}  } + J \qty{\color{orange}\qty{d\psi_t} \qty{\dd{v}{t}} + X_t(u) } - J X_t(u) &\text{by substitution} \\
&= \left(d \psi_{t}\right)\left(\frac{\partial v}{\partial s}\right)+J(u)\left(d \psi_{t}\right)\left(\frac{\partial v}{\partial t}\right) &\text{cancelling} \\
&= \left(d \psi_{t}\right)\left(\frac{\partial v}{\partial s} + 
{\color{red} \left( d \psi_{t}\right)^{-1} J(u)\left(d \psi_{t}\right)\left(\frac{\partial v}{\partial t}\right) }
\right) &\text{collecting terms}\\
&\definedas \left(d \psi_{t}\right)\left(\frac{\partial v}{\partial s} + 
{\color{red} \psi_t^* J(v) } 
\right)
&\text{by definition}
.\end{align*}

- Conclude that $v$ is a solution of
\begin{align*}
\frac{\partial v}{\partial s}+\psi_{t}^{\star} J(v) \frac{\partial v}{\partial t}=0
.\end{align*}

- Set $\varphi \definedas \psi_1$ and $J_1(v) \definedas \psi_1^* J(v)$ to obtain
\begin{align*}
\frac{\partial v}{\partial s}+ J_1(v) \frac{\partial v}{\partial t}=0
\end{align*}
of which $v$ is still a solution

- Property 1, Periodicity: attempt to check directly, using $\psi_{t+1} = \psi_t \circ \psi_1$:
\begin{align*}
v(s, t+1) &\definedas (\psi_t\inv \circ u)\qty{s, t + 1} \\
{}_?&= \qty{ \psi_1 \circ \psi_t\inv \circ u}(s, t) \\
&= \psi_1 \qty{ v(s, t)} \\
&\definedas \varphi(v(s,t))
.\end{align*}

> Just a guess. If the 1-parameter group is commutative then proving $\varphi(v(s, t-1)) = v(s, t)$ might work.

\newpage

- Recall definition of $v$:
  $$v(s, t) \definedas \psi_t\inv \qty{ u(s, t) }$$

- Verifying that $C(v) = C(u)$: not spelled out. Property of flow?
  - Need to check that $$\dd{u}{s}(s_0, t_0) = 0 \implies \dd{v}{s}(s_0, t_0) = 0$$
    where $$\dd{u}{s} = \qty{d\psi_t}\qty{\dd{v}{s}}$$
  - How: ?
- Verifying that $R(v) = R(u)$
  - Need to check that for $(s_0, t_0) \not \in C(u)$ and $s\neq s_0$ we have
    $$u(s_0,t_0) \neq u(s, t_0) \implies v(s_0, t_0) \neq v(s, t_0)$$
  - Follows directly: 
  \begin{align*}
  v(s_0, t_0) \neq v(s, t_0) 
&\iff \psi_t\inv(u(s_0, t_0)) \neq \psi_t\inv(u(s, t_0)) \quad\text{by definition}\\
&\iff \qty{\psi_t \circ \psi_t\inv} (u(s_0, t_0)) \neq \qty{\psi_t \circ \psi_t\inv} (u(s, t_0)) \quad\text{injectivity of }\psi_t \\
&\iff u(s_0, t_0) \neq u(s, t_0)
  .\end{align*}

$\qed$

\newpage

## Splitting the Main Theorem

- The main theorem is equivalent to two upcoming statements

Proposition (8.6.2: Statement 1, Critical Points are Discrete) 
:   Let $z = s + it$ where $(s, t) \in \RR^1 \cross S^1$ (?). 
    There exists a constant $\delta > 0$ such that 
    \begin{align*}
    0 < \abs{z} < \delta \implies \qty{dv}_z \neq 0
    .\end{align*}

Proof
: Postponed to p.264 because it relies on the 8.6.8 (Similarity Principle).

For the second statement, we set up some notation/definitions.

- $v\in C^\infty(\RR^2; W)$ is a solution satisfying
\begin{align*}
  \dd{v}{s} + J_1(v) \dd{v}{t} &= 0 \\ \\  v(s, t+1) &= \varphi(v(s, t)) \\ \\ C(v)=C(u),&~R(v) = R(u)
.\end{align*}



- The **regular points** are given by
\begin{align*}
R(v) = \theset{(s,t) \in \RR^2 \suchthat \dd{v}{s}(s, t) \neq 0, \quad v(s, t) \neq x^\pm(t),\quad v(s, t) \not\in v(\RR\setminus\theset{s}, t)  }
.\end{align*}

  > Note: last condition should be equivalent to $s\neq s' \implies v(s, t) \neq v(s', t)$.
  > For reference, also equivalent to $v(s, t) = v(s', t) \implies s = s'$.

\begin{center}
\includegraphics[width = 0.5\textwidth]{figures/image_2020-05-13-23-51-21.png} 
\end{center}

\newpage

- **Multiple points** are defined as follows:
  - Set $\bar \RR = \RR \disjoint \theset{\pm \infty}$
  - Extend $v: \RR^2 \to W$ to 
  \begin{align*}
  v: \bar \RR \cross \RR &\to W \\
  v(\pm \infty, t) &= x^\pm(t)
  .\end{align*}
  - Define the set of *multiple points* as 
  $$
  M(s, t) \definedas \theset{ (s', t) \in \RR^2 \suchthat s\neq s'\in \bar \RR, \quad v(s', t) = v(s, t) }
  $$
  
  > Note that the same $t$ is used throughout.


- Recast definition of $R(v)$ as "points in the complement of $C(v)$ that do not admit multiples".
  - Potentially incorrect formulation:
  \begin{align*}
  R(v) = C(v)^c \intersect_{(s, t) \in \bar \RR \cross \RR} M(s, t)^c
  .\end{align*}

  - Points to remember:
    - Condition 1, Nonzero $s\dash$derivative.
    - Condition 2, 

Proposition (8.6.3: Regular Points Open/Dense, \"Injectivity\")
:   Let $v$ be a smooth solution of the Cauchy-Riemann equation, then
    \begin{align*}
    \begin{rcases}
    v(s, t+1) = \varphi(v(s, t)) \\
    \dd{v}{s} \not\equiv 0
    \end{rcases}
    \implies R(v) \subseteq \RR^2 \quad\text{is open and dense}
    .\end{align*}

Proof (Long)
:   Splits into two parts:
     
    - Show $R(v)$ is open (easy)
    - Show $R(v)$ is dense (delicate)
  

## Regular Points Are Open

Proving the first part: $R(v)$ is open.

- Want to show $R(v)^c$ is closed.

- Toward a contradiction, suppose otherwise: $R(v)^c$ is *open*.
  - Use limit point definition: $R(v)^c$ is closed $\iff$ it contains all of its limit points
  - So $R(v)^c$ does *not* contain one of its limit points
  - Produces a sequence $$R(v)^c \supseteq \theset{(s_n, t_n)}_{n\in \NN} \converges{n\to\infty}\to (s, t) \in R(v)$$

\newpage

## Sequence is Bounded

- The first two conditions defining $R(v)$ are open conditions:
  - The two conditions: 
  \begin{align*}
  \dd{v}{s}(s, t) &\neq 0 &&\text{Condition 1}\\
  v(s, t) &\neq x^\pm(t) &&\text{Condition 2}
  .\end{align*}
  - Thus for $N\gg 1$ we have
  $$n\geq N \implies \dd{v}{s}(s_n, t_n) &\neq 0, \quad\quad v(s_n, t_n) \neq x^\pm(t)$$

> Note: what is an "open condition"?

- But $(s_n, t_n) \not\in R(v)$ for such $n$, so they must fail the last condition: injectivity 
  - Third condition:
  $$
  s \neq s' \implies v(s, t) \neq v(s', t)
  $$
  - Failing this conditions means:
  $$
  \forall n> N,~ \exists s_n' \in \RR \text{ s.t. } s'_n \neq s_n \qtext{and} v(s_n, t_n) = v(s_n', t_n).
  $$
- Produces a sequence $\theset{s_n'}_{n\in \NN}$, want to show it is bounded.
  - Toward a contradiction, suppose not, then there is a subsequence 
  $$\theset{s_{n_k}}_{n_k\in \NN} \converges{n_k \to\infty}\to \pm\infty.$$
  - This implies
  \begin{align*}
  v(s, t) 
&= \lim_{n_k \to \infty} v(s_{n_k}', t_{n_k}') \quad\quad\text{using continuity of } v\\
  &= v(\pm \infty, t) \\
  &\definedas x^\pm (t)
  .\end{align*}
  - Why? By definition, precisely because we extended $v$ by setting $v(\pm \infty, t) = x^{\pm}(t)$.
  - But condition 2 for points in $R(v)$ says $v(s, t) \neq x^\pm(t)$, so this contradicts $(s, t) \in R(v)$.

So the sequence is bounded.

\newpage

## Reaching a Contradiction

- Sequence is bounded, so apply Bolzano-Weierstrass to extract a convergent subsequence converging to some limit:
  \begin{align*}
  \theset{s_{n_j}'} \converges{n_j\to\infty}\to s'
  .\end{align*}
  - Use the fact that injectivity failed:
  \begin{align*}
\forall n,~ s'_n \neq s_n \qtext{and} v(s_n, t_n) &= v(s'_n, t_n) \\
\implies \lim_{n_k\to \infty} v(s_n, t_n) &= \lim_{n_k\to\infty} v(s'_n, t'_n) \\
\iff v(s, t)&= v(s', t) \hspace{6em}\text{using continuity}
  .\end{align*}
  - Use the fact that because $(s, t) \in R(v)$ we must have $$s = s'.$$

- *(Minor technical point)* Now have $\theset{s_{n_j}'}_{n_j \in \NN} \to s'$ and $\theset{s_n}_{n\in \NN} \to s$
  - Since the latter sequence is convergent, every subsequence converges to the same limit, so $\theset{s_{n_j}}_{n_j \in \NN} \to s$.

- Again using failed injectivity, i.e.
  \begin{align*}
    v(s, t) &= v(s', t) \\
    \implies v(s, t) - v(s', t) &= 0
  .\end{align*}
  we have 
  \begin{align*}
    s_{n_j}' \neq s_{n_j} \qtext{and} v(s_{n_j}, t_{n_j}) &= v(s_{n_j}', t_{n_j}) \\
  .\end{align*}

- In the last step, we do have equality in the limit, $s= s'$, and $\forall n_j$,
  \begin{align*}
    v(s_{n_j}, t_{n_j}) - v(s_{n_j}', t_{n_j}) &= 0, \\
    s_{n_j} - s_{n_j}' &\neq 0
  \end{align*}
  thus
  \begin{align*}
    \dd{v}{s}(s, t) = \lim_{n_j\to\infty} {v(s_{n_j}, t) - v(s_{n_j}', t) \over s_{n_j} - s_{n_j}'  } = 0
  .\end{align*}

- But $(s, t) \in R(v)$ and so this contradicts Condition 1.

This proves that $R(v)$ is open.
$\qed$

\newpage

Lemma 8.6.4 (Failure of Injectivity)
:   For every $r> 0$ there exists a $\delta >0$ such that 
    \begin{align*}
    \abs{t-t_0},~\abs{s-s_0} < \delta \implies \exists s' \in B_r(s_j) \text{ s.t. } v(s, t) = v(s', t)
    .\end{align*}

Proof
: Short, include.

Lemma (8.6.5: Unique Solutions in a Small Ball)
:   Let $v_1, v_2$ be two solutions of the CR-equation with $X_t \equiv 0$ on $B_\eps(0)$, $v_1(0, 0) = v_2(0, 0)$.

    \

    Suppose that $\qty{dv_1}_0, \qty{dv_2}_0 \neq 0$.
    Also suppose 
    \begin{align*}
    \forall \eps ~\exists \delta \text{ s.t. }
    \forall (s, t) \in B_{\delta}(0), ~\exists s'\in \RR 
    \begin{cases}
    (s', t) \in B_\eps(0) \\
    v_1(s, t) = v_2(s', t)
    \end{cases}
    .\end{align*}

    Then 
    \begin{align*}
    z\in B_\eps(0) \implies v_1(s, t) = v_2(s, t)
    .\end{align*}

Take perturbed CR equation:
\begin{align*}
\frac{\partial Y}{\partial s}+J_{0} \frac{\partial Y}{\partial t}+S \cdot Y=0
.\end{align*}

Fix $S\in C^\infty(\RR^2; \endo(\RR^{2n}))$



Lemma (Similarity Principle)
:   Let $Y \in C^\infty(B_\eps; \CC^n)$ be a solution to the perturbed CR equation and let $p>2$.
    Then there exists $0 < \delta < \eps$ and a map $A\in W^{1, p}(B_\delta, \gl(\RR^{2n}))$ and a holomorphic map $$\sigma: B_\delta \to \CC^n$$ such that 
    \begin{align*}
    \forall (s, t) \in B_\delta \quad Y(s, t) = A(s, t) ~ \sigma(s+it) \qtext{and} J_0 A(s, t) = A(s, t) J_0
    .\end{align*}

Use continuation principle to finish proofs of many old theorems/lemmas.

Theorem (8.6.11, Essential property of bar del)
:   For every $p>1$, the following operator is surjective and Fredholm:
    \begin{align*}
    \bar\del: W^{1, p}\qty{S^2; \CC^n} \to L^p(\Lambda^{0, 1} T^* S^2 \tensor \CC^n)
    .\end{align*}

Lead up to the proof of 8.1.5 in Section 8.7

# Goal 2: Continuation Principle
Goal 2: prove a continuation principle:

Proposition (8.6.6, Continuation Principle)
:   On an open $U \subset \RR^2$, let $Y$ be a solution to the perturbed CR equation
    \begin{align*}
    \dd{Y}{s} + J_0 \dd{Y}{t} + S\cdot Y = 0
    \end{align*}
    where $J_0$ is the standard complex structure on $\RR^{2n}$ and $S\in C^\infty(\RR^2, \endo(\RR^{2n}))$.
    \
    Say that $f$ has an *infinite-order zero* at $z_0$ iff 
    \begin{align*}
    \forall k\geq 0,\quad \sup_{\abs{z-z_0}\leq t} {\abs{f(z)} \over r^k} \converges{r\to 0}\to 0
    .\end{align*}

    > For $f$ smooth, equivalently $f^{(k)}(z_0) = 0$ for all $k$.

    Then the set
    \begin{align*}
    C \definedas \theset{(s, t) \in U \suchthat Y \text{ has an infinite order zero at } (s, t) }
    \end{align*}
    is clopen.
    In particular, if $U$ is connected and $Y = 0$ on some nonempty $V \subset U$, then $Y\equiv 0$.



Proposition (8.1.4, \"Transversality Property\")
:   \hfill 
    Define
    \begin{align*}
    \mathcal{Z}(x, y, J)\definedas 
    \left\{\left(u, H_{0}+h\right) | h \in \mathcal{C}_{\varepsilon}^{\infty}\left(H_{0}\right) \text { and } u \in \mathcal{M}(x, y, J, H)\right\}
    .\end{align*}
    If $(u, H_0 + h) \in \mathcal{Z}(x, y)$ then the following map admits a continuous right-inverse and is surjective:
    \begin{align*}
    \Gamma: W^{1, p}\left(\mathbb{R} \times S^{1} ; \mathbb{R}^{2 n}\right) \times \mathcal{C}_{\varepsilon}^{\infty}\left(H_{0}\right) & \longrightarrow L^{p}\left(\mathbb{R} \times S^{1} ; \mathbb{R}^{2 n}\right) \\
    (Y, h) & \longmapsto\left(d \mathcal{F}^{H_0 + h}\right)_{u}(Y)+\operatorname{grad}_{u} h
    \end{align*}

    where $\mcf^{H_0 + h}$ is the Floer operator corresponding to $H_+ h$.

    > Used to show (via the implicit function theorem) that $\mcz(x, y, J)$ is a Banach manifold when $x\neq y$.


