# Fall 2019


## 8

### a.

Let $\vector v \in \Lambda$, so $\vector v = \sum_{i=1}^n r_i \vector e_i$ where $r_i \in \ZZ$ for all $i$.

Then if $\vector x = \sum_{j=1}^n s_j \vector e_j \in \Lambda$ is arbitrary, we have $s_j \in \ZZ$ for all $j$ and 
\[
\inner{\vector v}{\vector x} 
&= \inner{\sum_{i=1}^n r_i \vector e_i}{\sum_{j=1}^n s_j \vector e_j } \\
&= \sum_{i=1}^n \sum_{j=1}^n r_i s_j \inner{\vector e_i}{\vector e_j }  \in \ZZ
\]

since this is a sum of products of integers (since $\inner{\vector e_i}{\vector e_j} \in \ZZ$ for each $i, j$ pair by assumption) so $\vector v \in \Lambda\dual$ by definition.

### b. 


**$\det M \neq 0$**:

Suppose $\det M = 0$. Then $\ker M \neq \vector 0$, so let $\vector v \in \ker M$ be given by $\vector v = \sum_{i=1}^n v_i \vector e_i \neq \vector 0$. 

Note that 
\[
M\vector v = 0 &\implies
\left[
\begin{array}{ccc}
\vector e_1 \cdot \vector e_1 & \vector e_1 \cdot \vector e_2 & \cdots \\
\vector e_2 \cdot \vector e_1 & \vector e_2 \cdot \vector e_2 & \cdots \\
\vdots & \vdots & \ddots
\end{array}
\right]
\left[\begin{array}{c}
v_1 \\ v_2 \\ \vdots
\end{array}\right] = \vector 0 \\ \\
&\implies \sum_{j=1}^n v_j\inner{\vector e_k}{\vector e_j} = 0 \qtext{for each fixed} k
.\]

We can now note that $\inner{\vector e_k}{\vector v} = \sum_{j=1}^n v_j \inner{\vector e_k}{\vector e_j} = 0$ for every $k$ by the above observation, which forces $\vector v = 0$ by non-degeneracy of $\inner{\wait}{\wait}$, a contradiction. 

$\qed$

*Alternative proof:*

Write $M = A^tA$ where $A$ has the $\vector e_i$ as columns. Then
\[
M\vector x = 0 
&\implies A^t A \vector x = 0 \\
&\implies \vector x^t A^t A \vector x = 0 \\
&\implies \norm{A \vector x}^2  = 0 \\
&\implies A\vector x = 0 \\
&\implies \vector x = 0
,\]

since $A$ has full rank because the $\vector e_i$ are linearly independent.

$\qed$

Let $A = [\vector e_1^t, \cdots, \vector e_n^t]$ be the matrix with $\vector e_i$ in the $i$th column.

**The rows of $A\inv$ span $\Lambda\dual$**:

Equivalently, the columns of $A^{-t}$ span $\Lambda\dual$.

Let $B = A^{-t}$ and let $\vector b_i$ denote the columns of $B$, so $\im B = \spanof{\theset{\vector b_i}}$.


Since $A \in \GL(n, \ZZ)$, $A\inv, A^t, A^{-t} \in \GL(n, \ZZ)$ as well.

\[
\vector v \in \Lambda\dual 
&\implies \inner{\vector e_i}{\vector v} = z_i \in \ZZ \quad \forall i \\
&\implies A^t \vector v = \vector z \definedas [z_1, \cdots, z_n] \in \ZZ^n \\
&\implies \vector v = A^{-t} \vector z \definedas B\vector z \in \im B \\
&\implies \vector v \in \im B \\
&\implies \Lambda\dual \subseteq \im B
,\]

and

\[
B^t A = (A^{-t})^t A = A\inv A = I \\
\implies \vector b_i \cdot \vector e_j = \delta_{ij} \in \ZZ \\
\implies \im B \subseteq \spanof~ \Lambda\dual
.\]

$\qed$

### c.

?
