
# Week 1

[Link to Notes](http://math.stanford.edu/~vakil/216blog/FOAGnov1817public.pdf)



## Exercise 1.3H: Right Exactness of Tensoring

Show that the following endofunctor
\[\begin{align*}
F: \rmod &\to \rmod \\
X &\mapsto X\tensor_R N \\
(X\mapsvia{f} Y) &\mapsto (X\tensor_R N \mapsvia{f \tensor \id_N} Y\tensor_R N)
\end{align*}\]
is exact.

Solution:

> Note: to make sense of the functor, we may need to show that there is an isomorphism $$\hom_{\rmod}(X, Y) \tensor_R \hom_{\rmod}(A, B) \to \hom_\rmod(X\tensor_R A, Y\tensor_R B).$$
> This is what makes taking $f:X\to Y$ and $g:A\to B$ and forming $f\tensor g: X\tensor A \to Y\tensor B$ well-defined?

Let $A\mapsvia{f} B \mapsvia{g} C \to 0$ be an exact sequence, so

- $\im f = \ker g$ by exactness at $B$
- $\im g = C$ by exactness at $C$.

Applying the above $F$ yields
\[
A\tensor_R N \mapsvia{f\tensor \id_N} B\tensor_R N \mapsvia{g\tensor \id_N} C\tensor_R N \to 0
\]

We thus need to show

1. Exactness as $C\tensor_R N$: $\im(g\tensor \id_N) = C\tensor_R N$, i.e. this is surjective.
2. Exactness at $B\tensor_R N$: $\im(f\tensor \id_N) = \ker(g\tensor id_N)$.

We'll use the fact that every element in a tensor product is a finite sum of elementary tensors.

- Claim: $\im(g\tensor \id_N) \subseteq C\tensor_R N$.
  - Let $b\tensor n \in B\tensor_R N$ be an elementary tensor
  - Then $(g\tensor \id_N)(b\tensor n) \definedas g(b) \tensor \id_N (n) = g(b) \tensor n$
  - Since $\im(g) = C$, there exists a $c\in C$ such that $g(b) = c$, so $g(b) \tensor n = c \tensor n \in C\tensor_R N$
  - Extend by linearity:

\begin{align*}
\qty{g\tensor_R \id_N}\qty{\sum_{i=1}^m r_i \cdot b_i \tensor n_i} =\sum_{i=1}^m (g\tensor \id_N)(r_i\cdot b_i \tensor n_i) \definedas \sum_{i=1}^m g(r_i\cdot b_i) \tensor \id_N(n_i) =_H \sum_{i=1}^m r_i\cdot c_i \tensor n_i \in C\tensor_R N
\end{align*}

  where we've used bilinearity for the first equality, and the equality marked with $H$ uses above the proof for elementary tensors, and noted that we can pull ring scalars $r_i\in R$ through $\rmod$ morphisms.
- Claim: $C \tensor_R N \subseteq \im(g\tensor \id_N)$.
  - Let $c\tensor n \in C\tensor_R N$ be an elementary tensor.
  - Then $c\in C = \im(g)$ implies $c = g(b)$ for some $b\in B$.
  - So $c\tensor n = g(b) \tensor n = (g\tensor \id_N)(b\tensor n) \in B\tensor_R N$.
  - Extend by linearity:
  \begin{align*}
  \sum_{i=1}^m r_i\cdot c_i \tensor n_i =_H \sum_{i=1}^m g(r_i\cdot b_i) \tensor n_i = \sum_{i=1}^m (g\tensor \id_N)(r_i\cdot b_i \tensor n_i) = (g\tensor \id_N)\qty{\sum_{i=1}^m r_i\cdot b_i \tensor n_i}
  .\end{align*}

This proves (1).

- Claim: $\im(f\tensor \id_N) \subseteq \ker(g\tensor \id_N)$.
  - Let $b\tensor n \in \im(f\tensor \id_N)$, we want to show $(g\tensor \id_N)(b\tensor n) = 0 \in C\tensor_R N$.
  - Then $b\tensor n = f(a)\tensor n$ for some $a\in A$.
  - By exactness of the original sequence, $\im f \subseteq \ker g$, so $g(f(a)) = 0 \in C$
  - Then
  \begin{align*}
  (g\tensor \id_N)\qty{ b \tensor n} = (g\tensor \id_N)(f(a)\tensor n) \definedas g(f(a)) \tensor n = 0\tensor n = 0\in C\tensor_R N
  \end{align*}
  where we've used the fact that $0\tensor x = 0$ in any tensor product.
  - Extend by linearity.

- Claim (**nontrivial part**): $\ker(g\tensor \id_N) \subseteq \im(f\tensor \id_N)$.

  > Note: the problem is that
  \begin{align*}
  x\in \ker(g\tensor \id_N) \implies x = \sum_{i=1}^m r_i\cdot b_i \tensor n_i \implies (g\tensor \id_N)\qty{\sum_{i=1}^m r_i\cdot b_i \tensor n_i} = \sum_{i=1}^m r_i\cdot g(b_i) \tensor n_i = 0\in C\tensor_R N
  \end{align*}
  **but** this does not imply that $g(b_i) = 0\in C$ for all $i$, which is what you would need to use $\im f = \ker g$ to write $g(b_i) = 0\implies \exists a_i, f(a_i) = b_i$ and pull everything back to $A\tensor_R N$.

  - Strategy: use the first claim and the first isomorphism theorem to obtain this situation:
  \begin{center}
  \begin{tikzcd}
{B\tensor_R N \over \im(f\tensor_R \id_N)} \ar[r, hook, "i"]\ar[rrr, bend left, dotted, "\alpha"] & {B\tensor_R N \over \ker(g \tensor_R \id_N)} \ar[r, "\cong"] & \im(g\tensor_R \id_N) \ar[equal]{r} & C\tensor_R N
  \end{tikzcd}
  \end{center}
  - The first injection $i$ will exist because $\im(g\tensor_R \id_N) \subseteq \ker(g\tensor_R \id_N)$ by the first claim.
  - The middle isomorphism is the first isomorphism theorem.
  - The RHS equality follows from surjectivity of $g\tensor_R \id_N$
  - We then apply a strengthened version of the 1st isomorphism theorem for modules:

  > Hungerford Ch.4 Thm 1.7: If $f:A\to B$ is a $R\dash$module morphism and $C\leq \ker f$ then there is a unique map $\tilde f: A/C\to B$ which is an isomorphism iff $f$ is an epimorphism and $C = \ker f$.
  >
  > Following Hungerford Ch.4 Prop. 5.4, p.210.

  - Since $\im(g\tensor_R \id_N)\subseteq \ker(g\tensor_R \id_N)$, by the theorem the map $\alpha$ exists and satisfies the same formula, i.e. $\alpha = \tilde g \tensor \tilde \id_N$ where the tilde denotes the induced map on quotients, so $\alpha([b\tensor n]) = g(b)\tensor n$.
    - We will show it is an isomorphism, which forces $\im(g\tensor_R \id_N) \cong \ker(g\tensor_R \id_N)$ by the above theorem.
  - Constructing the inverse map: define
  \begin{align*}
  \tilde \alpha\inv: C\times N &\to {B\tensor_R N \over \im(g\tensor_R \id_N) } \\
  (c, n) &\mapsto (b \tensor n)  \mod \im(g\tensor_R \id_N) \qtext{where} b \in g\inv(c)
  ,\end{align*}
  which we will show well-defined (i.e. independent of choice of $b$) and $R\dash$linear, lifting to a map $\alpha\inv$ out of the tensor product by the universal property which is a two-sided inverse for $\alpha$.

  - Well-defined:
    - $g\inv(b)$ exists because $g$ is surjective.
    - If $b\neq b'$ and $g(b') = 0$, then $0 = g(b) - g(b') = g(b-b')$ so $b-b' \in \ker g$.
    - By the original exactness, $b-b' \in \im f$ so $b-b' = f(a)$ for some $a\in A$.
    - Then $f(a) \tensor n \in \im(f\tensor \id)$ implies $f(a)\tensor n \equiv 0 \mod \im(f\tensor \id)$.
    - Then noting that $b-b' = f(a) \implies b = f(a) + b'$, working mod $\im(g\tensor_R \id_N)$ we have
    \begin{align*}
    b \tensor n \equiv (f(a) + b') \tensor n \equiv \qty{f(a) \tensor n} + \qty{b' \tensor n} \equiv b'\tensor n
    .\end{align*}
  - $R\dash$linear:
    - ?
  - Two-sided identity:
    - $(\alpha \circ \alpha\inv)(c\tensor n) = \alpha(b\tensor n) = g(b)\tensor n = c\tensor n$, so $\alpha\circ \alpha\inv = \id$.
    - $(\alpha\inv \circ \alpha)([b\tensor n]) = \alpha\inv(g(b) \tensor n) = [b'\tensor n]$ where $b'\in g\inv(g(b))$ implies $b'=b$, so $\alpha\circ\alpha\inv = \id$.

$\qed$
