# More Exercises 

## 1.3.K

> Note: I think this is an exercise about base change.

**Part a**: For $M$ an $A\dash$module and $\phi: A\to B$ a morphism of rings, give $B\tensor_A M$ the structure of a $B\dash$module and show that it describes a functor $A\dash\text{Mod}\to B\dash\text{Mod}$.


Solution

- $B\tensor_A M$ makes sense: $B$ is a $(B, A)\dash$bimodule with the usual multiplication on the left and the right action
\begin{align*}
A &\to \endo(B) \\
a &\mapsto (b\mapsto b\cdot \phi(a))
.\end{align*}

- $B\tensor_A M$ is a left $B\dash$module via the following action:
\begin{align*}
B &\to \endo(B\tensor_A M) \\
b_0 &\mapsto (b\tensor m \mapsto b_0 b \tensor m)
.\end{align*}

- This describes a functor:
\begin{align*}
F: A\dash\text{Mod} &\to B\dash\text{Mod} \\
X &\mapsto B\tensor_A X \\
(X\mapsvia{f} Y) &\mapsto (B\tensor_A X \mapsvia{\id_B \tensor f} B\tensor_A Y)
.\end{align*}

  - Need to check:
    - Preserves identity morphism, i.e. $X\in A\dash$Mod implies $F(\id_X) = \id_{F(X)}$ in $B\dash$Mod.
    - Preserves composition: $F(f\circ g) = F(f) \circ F(g)$.

- Preserving identity morphisms:
  - By construction $X\selfmap_{\id_X}$ maps to $B\tensor_A X \mapsvia{\id_B \tensor \id_X} B\tensor_A X$, can argue that this is the identity map for $B\dash$modules.
- Preserving composition:
\begin{align*}
(X\mapsvia{f} Y \mapsvia{g} Z) \mapsto (B\tensor_A X \mapsvia{ \id_B\tensor f} B\tensor_A Y \mapsvia{\id_B \tensor g} B\tensor_A Z) = (B\tensor_A X \mapsvia{\id_B \tensor (g\circ f)} B\tensor_A Z )
.\end{align*}

> Note: not sure if there's anything to show here.

**Part b**: If $\psi: A\to C$ is another ring morphism, show that $B\tensor_A C$ has a ring structure.


Solution:

- Note $B\tensor_A C$ makes sense, since $C$ is a left $A\dash$module via $a\mapsto (c\mapsto \psi(a)c)$.
- Need to define $(B\tensor_A C, P, M)$ such that it's an abelian group under $P$ (plus), a monoid under $M$ (multiplication), and left/right distributivity.
- Start by defining on cartesian products:
\begin{align*}
P: \qty{B\tensor_A C}^{\times 2} &\to B\tensor_A C \\
P\qty{ (b_1 \tensor c_1), (b_2\tensor c_2)} &= (b_1 +_B b_2) \tensor (c_1 +_C c_2)
,\end{align*}
\begin{align*}
M: \qty{B\tensor_A C}^{\times 2} &\to B\tensor_A C \\
M\qty{ (b_1 \tensor c_1),  (b_2\tensor c_2)} &= (b_1 \cdot_B b_2) \tensor (c_1 \cdot_C c_2)
.\end{align*}

- Check $A\dash$bilinearity:
\begin{align*}
P(a\cdot (b_1\tensor c_1),\, (b_2\tensor c_2)) 
&\definedas \qty{ a \cdot (b_1 + b_2)} \tensor (c_1 + c_2)  \\
&= \qty{ (b_1 + b_2)} \tensor a\cdot (c_1 + c_2) \quad\text{since $C$ is a left $A\dash$module} \\
&\definedas P((b_1\tensor c_1),\, a\cdot (b_2\tensor c_2)) 
.\end{align*}
\begin{align*}
M(a\cdot (b_1\tensor c_1),\, (b_2\tensor c_2)) 
&\definedas \qty{a\cdot (b_1 \cdot b_2)} \tensor (c_1 \cdot c_2) \\
&= (b_1 \cdot b_2) \tensor \qty{ a\cdot (c_1 \cdot c_2) } \quad\text{since $C$ is a left $A\dash$module} \\
&\definedas M((b_1\tensor c_1),\, a\cdot (b_2\tensor c_2)) 
.\end{align*}

- So these lift to maps out of $(B\tensor_A C)^{\tensor 2}$.
- $P$ forms an abelian group: clear because $+_B, +_C$ do, and commuting is just done within each factor.
- $M$ forms a monoid: clear for some reason.
- Checking distributivity, claim: it suffices to check on elementary tensors and extend by linearity?
 \begin{align*}
(b_0 \tensor c_0) \cdot \qty{(b_1 \tensor c_1) + (b_2\tensor c_2) } 
&= (b_0\tensor c_0) \cdot \qty{ (b_1 + b_2) \tensor (c_1 + c_2) } \\
&= (b_0(b_1 + b_2)) \tensor ( c_0(c_1 + c_2)) \\
&= (b_0 b_1 + b_0 b_2) \tensor (c_0 c_1 + c_0 c_2) \\
&= \cdots
 .\end{align*}


## 1.3.L

If $S\subseteq A$ is multiplicative and $M\in A\dash$Mod, describe a natural isomorphism
\begin{align*}
\eta: (S\inv A)\tensor_A M \to (S\inv M)
\end{align*}
as both $S\inv A\dash$modules and $A\dash$modules.

Solution

- Recall the definition
\begin{align*}
S\inv A\definedas \theset{ {a\over s} \suchthat a\in A, s\in S} / \sim \\
{a_1 \over s_1} \sim {a_2 \over s_2} \iff \exists s\in S \text{ such that } s\qty{ s_2 a_1 - s_1 a_2 } = 0_A
.\end{align*}
- Similarly $S\inv M = \theset{{m\over s}}/\sim$.

The universal property: in $A\dash$Mod, $M\to S\inv M$ is initial among all morphisms $\alpha: M\to N$ such that $\alpha(S) \subseteq N\units$:
\begin{center}
\begin{tikzcd}
& S\inv M \ar[d, dotted, "{\exists ! \tilde\alpha}"] \\
M\ar[ru, "S\inv \cdot"]\ar[r, "\alpha"] & N 
\end{tikzcd}
\end{center}

> Strategy: define a map $M\to S\inv A \tensor_A M$ such that $S$ is invertible in the image to obtain a map?
> Show they satisfy the same universal property?

- Since $M \in A\dash$Mod, we have an action $a\cdot m$, so define 
\begin{align*}
\eta: (S\inv A)\times M &\to (S\inv M) \\
\qty{ {a\over s}, m } &\mapsto {a\cdot m \over s }
.\end{align*}

- The tensor product $S\inv A \tensor_A M$ makes sense.
  - $S\inv A$ is a right $A\dash$module by $a_0 \mapsto \qty{ {a\over s} \mapsto {a_0 a \over s}}$.
  - $S\inv M$ is a left $A\dash$module by $a_0 \mapsto (m \mapsto a_0 \cdot m)$ where the action comes from the $A\dash$module structure of $M$.
- The map makes sense as an $A\dash$module morphism
  - $S\inv A \tensor_A M$ is a left $A\dash$module by $a_0 \mapsto \qty{{a\over s}\tensor m \mapsto {a_0 a \over s} \tensor m}$
  - $S\inv M$ is a left $A\dash$module by $a_0 \mapsto \qty{ {m\over s } \mapsto {a_0 \cdot m \over s}}$ using the $A\dash$module structure on $M$.
- The map makes sense as an $S\inv A\dash$module morphism
  - $S\inv A \tensor_A M$ is a left $S\inv A\dash$module by ${a_0\over s_0} \mapsto \qty{ {a\over s}\tensor m \mapsto {a_0 a \over s_0 s} \tensor m }$
  - $S\inv M$ is a left $S\inv A\dash$module by ${a_0\over s_0} \mapsto \qty{{m \over s} \mapsto {a_0 \cdot m \over s_0 s}  }$ by the $A\dash$module structure on $M$. 

- Well-defined: ?
- $A\dash$bilinear: let $r\in A$, then
 \begin{align*}
\eta\qty{r \cdot {a\over s}, m} 
&\definedas \eta\qty{{r\cdot a\over s}, m}  \\
&\definedas {\psi(r\cdot a)(m) \over s} \\
&= {r\cdot \psi(a)(m) \over s} \quad\text{since $\psi$ is a ring morphism} \\
&= {\psi(a)(r\cdot m) \over s} \quad\text{since $\psi(a)$ is a ring morphism} \\
&\definedas \eta\qty{ {a\over s}, r\cdot m}
 .\end{align*}
  So this lifts to a map out of the tensor product.

- $S\inv A\dash$bilinear?

## 1.3.P

Show that the fiber product over the terminal object is the cartesian product.

Solution:

- Recall definition: $T$ is terminal iff every object $X$ admits a morphism $X\to T$.
- Strategy: use both universal products to produce an isomorphism
- Let $\pr_X, \pr_Y$ by the cartesian product projections, and $\pr_X^T, \pr_Y^T$ be the fiber product projections
- Let $T_X, T_Y$ be the maps $X\to T, Y\to T$.
- Since $X\cross Y$ is an object in this category, it admits one unique map to $T$

\begin{center}
\begin{tikzcd}
X\cross Y\ar[r, "\pr_Y"]\ar[d, "\pr_X"']\ar[dr, "T_{X\cross Y}"] & Y\ar[d, "T_Y"] \\
X\ar[r, "T_X"'] & T 
\end{tikzcd}
\end{center}

- But now $T_Y \circ \pr_Y: X\cross Y \to T$ is another such map, so it must equal $T_{X\cross Y}$.
- Similarly $T_X \circ \pr_X$ is equal to $T_{X\cross Y}$. 
- Thus $T_Y \circ \pr_Y = T_X \circ \pr_Y$, which is part of the universal property for $X\cross_T Y$.
- By the universal property of $X\cross Y$, for every $W$ admitting maps to $X, Y$ we get the following $h_0$:
\begin{center}
\begin{tikzcd}
W \ar[drr, bend left]\ar[rdd, bend right]\ar[dr, dotted, "\exists ! h_0"] & & \\
& X\cross Y\ar[r, "\pr_Y"]\ar[d, "\pr_X"] & Y\ar[d, "T_Y"] \\
& X\ar[r, "T_X"] & T 
\end{tikzcd}
\end{center}
> Note that $T$ doesn't matter in this particular diagram.

- This gives us the LHS diagram, the RHS comes from the universal property of $X\cross Y$:
\begin{center}
\begin{tikzcd}
X\cross_T Y\ar[drr, "\pr_Y^T", bend left]\ar[rdd, "\pr_X^T", bend right]\ar[dr, dotted, "\exists ! h_0"] & & \\
& X\cross Y\ar[r, "\pr_Y"]\ar[d, "\pr_X"] & Y\ar[d, "T_Y"] \\
& X\ar[r, "T_X"] & T 
\end{tikzcd}
\begin{tikzcd}
X\cross Y\ar[drr, "\pr_Y", bend left]\ar[rdd, "\pr_X", bend right]\ar[dr, dotted, "\exists ! h_1"] & & \\
& X\cross_T Y\ar[r, "\pr_Y^T"]\ar[d, "\pr_X^T"] & Y\ar[d, "T_Y"] \\
& X\ar[r, "T_X"] & T 
\end{tikzcd}
\end{center}




- By commutativity, $h_0 \circ h_1 = \id_{X\cross Y}$ and vice-versa?


## 1.3.Q

Show that if the two squares in this diagram are cartesian, then then outer square is also cartesian:
\begin{center}
\begin{tikzcd}
U \ar[r]\ar[d] & V\ar[d] \\
W \ar[r]\ar[d] & X\ar[d] \\
Y \ar[r] & Z
\end{tikzcd}
\end{center}


Solution:

- Need to show that given two maps $R\to V$ and $R\to Y$ such that $(V\to Z) \circ (U\to V) = (Y\to Z) \circ (R\to Y)$, then there is a unique map $R\to U$ giving a commuting diagram:
\begin{center}
\begin{tikzcd}
U\ar[drr, bend left] \ar[rdd, bend right] & & \\
& R\ar[ul, dotted, "\exists !\, ?"] \ar[r]\ar[d] & V\ar[d] \\
 & Y \ar[r] & Z
\end{tikzcd}
\end{center}

- Applying the bottom square:
  - Need to produce maps $R\to X$ and $R\to Y$
  - We're given a map $R\to Y$ by assumption.
  - We can build a map $R\to X$ by taking $(V\to X) \circ (R\to V)$.
  - We then get a map $R\to W$:
\begin{center}
\begin{tikzcd}
W\ar[drr, bend left] \ar[rdd, bend right] & & \\
& R\ar[ul, dotted, "\exists !"] \ar[r]\ar[d] & X\ar[d] \\
 & Y \ar[r] & Z
\end{tikzcd}
\end{center}

- Applying the top square:
  - We have a map $R\to V$ by assumption
  - We have a map $R\to W$ from step 1
  - We have maps $V\to X$ and $W\to X$ from the top square
  - We thus obtain
\begin{center}
\begin{tikzcd}
U\ar[drr, bend left] \ar[rdd, bend right] & & \\
& R\ar[ul, dotted, "\exists !"] \ar[r]\ar[d] & V\ar[d] \\
 & W \ar[r] & X
\end{tikzcd}
\end{center}
