# Spring 2020


## 1

Concepts used:

- DCT
- Weierstrass Approximation Theorem

**Solution**:

- Suppose $p$ is a polynomial, then
\begin{align*}
\lim_{k\to\infty} \int_0^1 kx^{k-1} p(x) \, dx
&= \lim_{k\to\infty} \int_0^1 \qty{ \dd{}{x}x^k } p(x) \, dx \\
&= \lim_{k\to\infty} \left[ x^k p(x) \evalfrom_0^1 - \int_0^1 x^k \qty{\dd{}{x} p(x) } \, dx \right] \quad\text{integrating by parts}\\
&= p(1) - \lim_{k\to\infty} \int_0^1 x^k \qty{\dd{}{x} p(x) } \, dx
,\end{align*}

- Thus it suffices to show that
\begin{align*}
\lim_{k\to\infty} \int_0^1 x^k \qty{\dd{}{x} p(x) } \, dx = 0
.\end{align*}

- Integrating by parts a second time yields
\begin{align*}
\lim_{k\to\infty} 
\int_0^1 x^k \qty{\dd{}{x} p(x) } \, dx
&= \lim_{k\to\infty} 
{x^{k+1} \over k+1} p'(x) \evalfrom_0^1 - \int_0^1 {x^{k+1} \over k+1} \qty{ \dd{^2}{x^2}p(x)} \, dx \\
&= - \lim_{k\to\infty} \int_0^1 {x^{k+1} \over k+1} \qty{ \dd{^2}{x^2}p(x)} \, dx \\
&= - \int_0^1 \lim_{k\to\infty}  {x^{k+1} \over k+1} \qty{ \dd{^2}{x^2}p(x)} \, dx \quad\text{by DCT} \\
&= - \int_0^1 0 \qty{ \dd{^2}{x^2}p(x)} \, dx \\
&= 0
.\end{align*}

  - The DCT can be applied here because $f''$ is continuous and $[0, 1]$ is compact, so $f''$ is bounded on $[0, 1]$ by a constant $M$ and 
  $$\int_0^1 \abs{x^k f''(x)} \leq \int_0^1 1\cdot M = M < \infty.$$

- Now use the Weierstrass approximation theorem: 
  - If $f: [a, b] \to \RR$ is continuous, then for every $\eps>0$ there exists a polynomial $p_\eps(x)$ such that $\norm{f - p_\eps}_\infty < \eps$.

- Thus 
\begin{align*}
\abs{ \int_0^1 kx^{k-1} p_\eps(x)\,dx - \int_0^1 kx^{k-1}f(x)\,dx  } 
&= \abs{ \int_0^1 kx^{k-1} \qty{p_\eps(x) - f(x)} \,dx  } \\
&\leq \abs{ \int_0^1 kx^{k-1} \norm{p_\eps-f}_\infty \,dx  } \\
&= \norm{p_\eps-f}_\infty \cdot \abs{ \int_0^1 kx^{k-1} \,dx  } \\
&= \norm{p_\eps-f}_\infty \cdot x^k \evalfrom_0^1 \\
&= \norm{p_\eps-f}_\infty \converges{\eps\to 0}\to 0
\end{align*}

  and the integrals are equal. 

- By the first argument, $$\int_0^1 kx^{k-1} p_\eps(x) \,dx = p_\eps(1) \text{ for each } \eps$$ 
- Since uniform convergence implies pointwise convergence, $p_\eps(1) \converges{\eps\to 0}\to f(1)$.


## 2

Concepts used:

- Definition of outer measure: $m_*(E) = \inf_{\theset{Q_j} \covers E} \sum \abs {Q_j}$ where $\theset{Q_j}$ is a countable collection of closed cubes.
- Break $\RR$ into $\disjoint_{n\in \ZZ} [n, n+1)$, each with finite measure.
- Theorem: $m_*(Q) = \abs{Q}$ for $Q$ a closed cube (i.e. the outer measure equals the volume).

Proof (of Theorem)
:   Statement: if $Q$ is a closed cube, then $m_*(Q) = \abs{Q}$, the usual volume.

    - $m_*(Q) \leq \abs{Q}$:
      - Since $Q\subseteq Q$, $Q\covers Q$ and $m_*(Q) \leq \abs{Q}$ since $m_*$ is an infimum over such coverings.
    - $\abs{Q} \leq m_*(Q)$:
      - Fix $\eps > 0$.
      - Let $\theset{Q_i}_{i=1}^\infty \covers Q$ be arbitrary, it suffices to show that 
          $$\abs{Q} \leq \qty{\sum_{i=1}^\infty \abs{Q_i}} + \eps.$$
      -  Pick open cubes $S_i$ such that $Q_i\subseteq S_i$ and $\abs{Q_i} \leq \abs{S_i} \leq (1+\eps)\abs{Q_i}$.
      - Then $\theset{S_i} \covers Q$, so by compactness of $Q$ pick a finite subcover with $N$ elements.

      - Note 
      \begin{align*}
      Q \subseteq \union_{i=1}^N S_i \implies \abs{Q} \leq \sum_{i=1}^N \abs{S_i} \leq \sum_{i=1}^N (1+\eps) \abs{Q_j} \leq (1+\eps)\sum_{i=1}^\infty \abs{Q_i } 
      .\end{align*}
      - Taking an infimum over coverings on the RHS preserves the inequality, so 
        $$\abs{Q} \leq (1+\eps) m_*(Q)$$
      - Take $\eps\to 0$ to obtain final inequality.


### a

- If $m_*(E) = \infty$, then take $B = \RR^n$ since $m(\RR^n) = \infty$.
- Suppose $N \definedas m_*(E) < \infty$.

- Since $m_*(E)$ is an infimum, by definition, for every $\eps> 0$ there exists a covering by closed cubes $\theset{Q_i(\eps)}_{i=1}^\infty \covers E$ depending on $\eps$ such that 
$$
\sum_{i=1}^\infty \abs{Q_i(\eps)} < N + \eps
.$$

- For each fixed $n$, set $\eps_n = {1\over n}$ to produce such a covering $\theset{Q_i(\eps_n)}_{i=1}^\infty$ and set $B_n \definedas \union_{i=1}^\infty Q_i(\eps_n)$.

- The outer measure of cubes is *equal* to the sum of their volumes, so 
\begin{align*}
m_*(B_n) = \sum_{i=1}^\infty \abs{Q_i(\eps_n)} < N + \eps_n = N + {1\over n}
.\end{align*}

- Now set $B \definedas \intersect_{n=1}^\infty B_n$.

  - Since $E\subseteq B_n$ for every $n$, $E\subseteq B$
  - Since $B$ is a countable intersection of countable unions of closed sets, $B$ is Borel.
  - Since $B_n \subseteq B$ for every $n$, we can apply subadditivity to obtain the inequality
  \begin{align*}
  E \subseteq B \subseteq B_n \implies
  N \leq m_*(B) \leq m_*(B_n) < N + {1\over n} \qtext{for all} n\in \ZZ^{\geq 1}
  .\end{align*}

- This forces $m_*(E) = m_*(B)$.


### b

Suppose $m_*(E) < \infty$.

- By (a), find a Borel set $B\supseteq E$ such that $m_*(B) = m_*(E)$
- Note that $E\subseteq B \implies B\intersect E = E$ and $B\intersect E^c = B\setminus E$.
- By assumption, 
\begin{align*}
m_*(B) &= m_*(B\intersect E) + m_*(B\intersect E^c) \\
m_*(E) &= m_*(E) + m_*(B\setminus E) \\ 
m_*(E) - m_*(E) &= m_*(B\setminus E) \qquad\qquad\text{since } m_*(E) < \infty \\ 
\implies m_*(B\setminus E) &= 0
.\end{align*}
- So take $N = B\setminus E$; this shows $m_*(N) = 0$ and $E = B\setminus (B\setminus E) = B\setminus N$.


If $m_*(E) = \infty$:

- Apply result to $E_R\definedas E \intersect [R, R+1)^n \subset \RR^n$ for $R\in \ZZ$, so $E = \disjoint_R E_R$
- Obtain $B_R, N_R$ such that $E_R = B_R \setminus N_R$, $m_*(E_R) = m_*(B_R)$, and $m_*(N_R) = 0$.
- Note that
  -   $B\definedas \union_R B_R$ is a union of Borel sets and thus still Borel
  -  $E = \union_R E_R$
  - $N\definedas B\setminus E$
  - $N' \definedas \union_R N_R$ is a union of null sets and thus still null
- Since $E_R \subset B_R$ for every $R$, we have $E\subset B$
- We can compute
\begin{align*}
N = B\setminus E = \qty{ \union_R B_R } \setminus \qty{\union_R E_R } \subseteq \union_R \qty{B_R\setminus E_R} = \union_R N_R \definedas N'
\end{align*}
where $m_*(N') = 0$ since $N'$ is null, and thus subadditivity forces $m_*(N) = 0$.

## 3

Concepts used:

- Limits
- Cauchy Criterion for Integrals: $\int_a^\infty f(x) \,dx$ converges iff for every $\eps>0$ there exists an $M_0$ such that $A,B\geq M_0$ implies $\abs{\int_A^B f} < \eps$, i.e. $\abs{\int_A^B f} \converges{A\to\infty}\to 0$.
- Integrals of $L^1$ functions have vanishing tails: $\int_{N}^\infty \abs{f} \converges{N\to\infty}\to 0$.
- Mean Value Theorem for Integrals: $\int_a^b f(t)\, dt = (b-a) f(c)$ for some $c\in [a, b]$.

### a

Stated integral equality: 

- Let $\eps > 0$
- $C_c(\RR^n) \injects L^1(\RR^n)$ is dense so choose $\theset{f_n} \to f$ with $\norm{f_n - f}_1 \to 0$.
- Since $\theset{f_n}$ are compactly supported, choose $N_0\gg 1$ such that $f_n$ is zero outside of $B_{N_0}(\vector 0)$.
- Then
\begin{align*}
N\geq N_0 \implies \int_{\abs x > N} \abs{f} &= \int_{\abs x > N} \abs{f - f_n + f_n} \\
&\leq \int_{\abs x > N} \abs{f-f_n} + \int_{\abs x > N} \abs{f_n} \\
&= \int_{\abs x > N} \abs{f-f_n} \\ 
&\leq \int_{\abs x > N} \norm{f-f_n}_1 \\
&= \norm{f_n-f}_1 \qty{\int_{\abs x > N} 1} \\
&\converges{n\to\infty}\to 0 \qty{\int_{\abs x > N} 1} \\
&= 0\\
&\converges{N\to\infty}\to 0
.\end{align*}


To see that this doesn't force $f(x)\to 0$ as $\abs{x} \to \infty$:

- Take $f(x)$ to be a train of boxes of height 1 and area $1/2^j$ centered on even integers.
- Then $$\int_{\abs x > N} \abs{f} = \sum_{j=N}^\infty 1/2^j \converges{N\to\infty}\to 0$$ as the tail of a convergent sum. 
- However $f(x) = 1$ for infinitely many even integers $x > N$, so $f(x) \not\to 0$ as $\abs{x}\to\infty$.

### b

#### Solution 1 ("Trick")

- Since $f$ is decreasing on $[1, \infty)$, for any $t\in [x-n, x]$ we have
\begin{align*}
x-n \leq t \leq x \implies f(x) \leq f(t) \leq f(x-n)
.\end{align*}

- Integrate over $[x, 2x]$, using monotonicity of the integral:
\begin{align*}
\int_x^{2x} f(x) \,dt \leq 
\int_x^{2x} f(t) \,dt \leq 
\int_x^{2x} f(x-n) \,dt \\ 
\implies 
f(x) \int_x^{2x} \,dt \leq 
\int_x^{2x} f(t) \,dt \leq 
f(x-n) \int_x^{2x} \,dt  \\
\implies xf(x) \leq \int_x^{2x} f(t) \, dt \leq xf(x-n)
.\end{align*}

- By the Cauchy Criterion for integrals, $\lim_{x\to \infty} \int_x^{2x} f(t)~dt = 0$.
- So the LHS term $\lim_{x\to \infty} xf(x) = 0$.
- Since $x>1$, $\abs{f(x)} \leq \abs{xf(x)}$ 
- Thus $f(x) \to 0$ as well.

#### Solution 2 (Variation on the Trick)

- Use mean value theorem for integrals:
\begin{align*}
\int_x^{2x} f(t)\, dt = xf(c_x) \quad\text{for some $c_x \in [x, 2x]$ depending on $x$}
.\end{align*}

- Since $f$ is decreasing, 
\begin{align*}
x\leq c_x \leq 2x 
&\implies f(2x)\leq f(c_x) \leq f(x) \\
&\implies 2xf(2x)\leq 2xf(c_x) \leq 2xf(x) \\
&\implies 2xf(2x)\leq 2x\int_x^{2x} f(t)\, dt \leq 2xf(x) \\
.\end{align*}

- By Cauchy Criterion, $\int_x^{2x} f \to 0$.
- So $2x f(2x) \to 0$, which by a change of variables gives $uf(u) \to 0$.
- Since $u\geq 1$, $f(u) \leq uf(u)$ so $f(u) \to 0$ as well.

#### Solution 3 (Contradiction)
\hfill
Just showing $f(x) \converges{x\to \infty}\to 0$:

- Toward a contradiction, suppose not.
- Since $f$ is decreasing, it can not diverge to $+\infty$
- If $f(x) \to -\infty$, then $f\not\in L^1(\RR)$: choose $x_0 \gg 1$ so that $t\geq x_0 \implies f(t) < -1$, then 
- Then $t\geq x_0 \implies \abs{f(t)} \geq 1$, so
 \begin{align*}
\int_1^\infty \abs{f} \geq \int_{x_0}^\infty \abs{f(t) } \, dt \geq \int_{x_0}^\infty 1 =\infty
 .\end{align*}

- Otherwise $f(x) \to L\neq 0$, some finite limit.
- If $L>0$:
  - Fix $\eps>0$, choose $x_0\gg 1$ such that $t\geq x_0 \implies L-\eps \leq f(t) \leq L$
  - Then $$\int_1^\infty f \geq \int_{x_0}^\infty f \geq \int_{x_0}^\infty \qty{L-\eps}\,dt = \infty$$
- If $L<0$:
  - Fix $\eps > 0$, choose $x_0\gg 1$ such that $t\geq x_0 \implies L \leq f(t) \leq L + \eps$.
  - Then $$\int_1^\infty f \geq \int_{x_0}^\infty f \geq \int_{x_0}^\infty \qty{L}\,dt = \infty$$

Showing $xf(x) \converges{x\to \infty}\to 0$.

- Toward a contradiction, suppose not.
- (How to show that $xf(x) \not\to + \infty$?)
- If $xf(x)\to -\infty$
  - Choose a sequence $\Gamma = \theset{\hat x_i}$ such that $x_i \to \infty$ and $x_i f(x_i) \to -\infty$.
  - Choose a subsequence $\Gamma' = \theset{x_i}$ such that $x_if(x_i) \leq -1$ for all $i$ and $x_i \leq x_{i+1}$.
  - Choose a further subsequence $S = \theset{x_i \in \Gamma' \suchthat 2x_i  < x_{i+1}}$.
  - Then since $f$ is always decreasing, for $t\geq x_0$, $\abs f$ is increasing, and $\abs{f(x_i)} \leq \abs{f(2x_i)}$, so
  \begin{align*}
  \int_1^{\infty} \abs{f} \geq \int_{x_0}^\infty \abs{f} \geq \sum_{x_i \in S} \int_{x_i}^{2x_i} \abs{f(t)} \, dt \geq 
  \sum_{x_i \in S} \int_{x_i}^{2x_i} \abs{f(x_i)} &= \sum_{x_i \in S} x_i f(x_i) \to \infty
  .\end{align*}

- If $xf(x) \to L \neq 0$ for $0 < L< \infty$:
  - Fix $\eps> 0$, choose an infinite sequence $\theset{x_i}$ such that $L-\eps \leq x_i f(x_i) \leq L$ for all $i$.
\begin{align*}
\int_1^\infty \abs{f} \geq \sum_S \int_{x_i}^{2x_i} \abs{f(t)}\,dt \geq \sum_S \int_{x_i}^{2x_i} f(x_i) \,dt = \sum_S x_i f(x_i) \geq \sum_S \qty{L-\eps} \to \infty
.\end{align*}
- If $xf(x) \to L \neq 0$ for $-\infty < L < 0$:
  - Fix $\eps> 0$, choose an infinite sequence $\theset{x_i}$ such that $L \leq x_i f(x_i) \leq L + \eps$ for all $i$.
\begin{align*}
\int_1^\infty \abs{f} \geq \sum_S \int_{x_i}^{2x_i} \abs{f(t)}\,dt \geq \sum_S \int_{x_i}^{2x_i} f(x_i) \,dt = \sum_S x_i f(x_i) \geq \sum_S \qty{L} \to \infty
.\end{align*}

#### Solution 4 (Akos's Suggestion)

For $x\geq 1$, 
\begin{align*}
\abs{xf(x)} = \abs{ \int_x^{2x} f(x) \, dt } \leq \int_x^{2x} \abs{f(x)} \, dt \leq \int_x^{2x} \abs{f(t)}\, dt \leq \int_x^{\infty} \abs{f(t)} \,dt \converges{x\to\infty}\to 0
\end{align*}
  where we've used 
  
  - Since $f$ is decreasing and $\lim_{x\to\infty}f(x) =0$ from part (a), $f$ is non-negative.
  - Since $f$ is positive and decreasing, for every $t\in[a, b]$ we have $\abs{f(a)} \leq \abs{f(t)}$.
  - By part (a), the last integral goes to zero.

#### Solution 5 (Peter's)

- Toward a contradiction, produce a sequence $x_i\to\infty$ with $x_i f(x_i) \to \infty$ and $x_if(x_i) > \eps > 0$, then
\begin{align*}
\int f(x) \, dx 
&\geq \sum_{i=1}^\infty \int_{x_i}^{x_{i+1}} f(x) \, dx \\
&\geq \sum_{i=1}^\infty \int_{x_i}^{x_{i+1}} f(x_{i+1}) \, dx \\
&=    \sum_{i=1}^\infty f(x_{i+1}) \int_{x_i}^{x_{i+1}} \, dx \\
&\geq \sum_{i=1}^\infty (x_{i+1} - x_i) f(x_{i+1}) \\
&\geq \sum_{i=1}^\infty (x_{i+1} - x_i) {\eps \over x_{i+1}} \\
&= \eps \sum_{i=1}^\infty \qty{ 1 - {x_{i-1} \over x_i}} \to \infty
\end{align*}
  which can be ensured by passing to a subsequence where $\sum {x_{i-1} \over x_i} < \infty$.

### c

- No: take $f(x) = {1\over x\ln x}$
- Then by a $u\dash$substitution,
  \begin{align*}
  \int_0^x f = \ln\qty{\ln (x)} \converges{x\to\infty}\to \infty
  \end{align*}
  is unbounded, so $f\not\in L^1([1, \infty))$.
- But 
  \begin{align*}
  xf(x) = { 1 \over \ln(x)} \converges{x\to\infty} \to 0
  .\end{align*}


## 4

Relevant concepts:

- Tonelli: non-negative and measurable yields measurability of slices and equality of iterated integrals
- Fubini: $f(x, y) \in L^1$ yields *integrable* slices and equality of iterated integrals
- F/T: apply Tonelli to $\abs{f}$; if finite, $f\in L^1$ and apply Fubini to $f$

\begin{align*}
\norm{H(x)}_1 
&= \int_\RR \abs{H(x, y)} \, dx \\
&= \int_\RR \abs{ \int_\RR f(y)g(x-y) \,dy } \, dx \\
&\leq \int_\RR \qty{ \int_\RR \abs{f(y)g(x-y)}  \, dy } \, dx \\
&= \int_\RR \qty{ \int_\RR \abs{f(y)g(x-y)}  \, dx} \, dy \quad\text{by Tonelli} \\
&= \int_\RR \qty{ \int_\RR \abs{f(y)g(t)}  \, dt} \, dy \quad\text{setting } t=x-y, \,dt = - dx \\
&= \int_\RR \qty{ \int_\RR \abs{f(y)}\abs{g(t)}  \, dt}\, dy \\
&= \int_\RR \abs{f(y)} \qty{ \int_\RR \abs{g(t)}  \, dt}\, dy \\
&\definedas \int_\RR \abs{f(y)} \cdot \norm{g}_1 \,dy \\
&= \norm{g}_1 \int_\RR \abs{f(y)} \,dy \\
&\definedas \norm{g}_1 \norm{f}_1  \\
&< \infty \qtext{by assumption}
.\end{align*}

- $H$ is measurable on $\RR^2$:
  - If we can show $\tilde f(x, y) \definedas f(y)$ and $\tilde g(x, y) \definedas g(x-y)$ are both measurable on $\RR^2$, then $H = \tilde f \cdot \tilde g$ is a product of measurable functions and thus measurable. 
  - $f \in L^1$, and $L^1$ functions are measurable by definition.
  - The function $(x, y) \mapsto g(x-y)$ is measurable on $\RR^2$:
    - Let $g$ be measurable on $\RR$, then the cylinder function $G(x, y) = g(x)$ on $\RR^2$ is always measurable
    - Define a linear transformation $T \definedas \thevector{1, -1; 0, 1}$ which sends $(x,y) \to (x-y, y)$, then $T\in \GL(2, \RR)$ is linear and thus measurable.
    - Then $(G\circ T)(x, y) = G(x-y, y) = \tilde g(x-y)$, so $\tilde g$ is a composition of measurable functions and thus measurable.

- Apply **Tonelli** to $\abs{H}$
  - $H$ measurable implies $\abs{H}$ is measurable
  - $\abs{H}$ is non-negative
  - So the iterated integrals are equal in the extended sense
  - The calculation shows the iterated integral is finite, to $\int \abs{H}$ is finite and $H$ is thus integrable on $\RR^2$.

> Note: Fubini is not needed, since we're not calculating the actual integral, just showing $H$ is integrable.

## 5 

Concepts used:

- DCT
- Passing limits through products and quotients

Note that 
\begin{align*}
\lim_{n} \qty{1 + {x^2 \over n}}^{-(n+1)} 
&= {1 \over \lim_{n} \qty{1 + {x^2 \over n}}^1 \qty{1 + {x^2 \over n}}^n } \\
&= {1 \over 1 \cdot e^{x^2}} \\
&= e^{-x^2}
.\end{align*}

If passing the limit through the integral is justified, we will have
\begin{align*}
\lim_{n\to\infty} \int_0^n \qty{ 1 + {x^2\over n}}^{-(n+1)}\, dx 
&= \lim_{n\to\infty} \int_\RR \chi_{[0, n]} \qty{ 1 + {x^2\over n}}^{-(n+1)} \, dx  \\
&= \int_\RR \lim_{n\to\infty} \chi_{[0, n]} \qty{ 1 + {x^2\over n}}^{-(n+1)} \, dx  \qtext{by the DCT} \\
&= \int_\RR \lim_{n\to\infty} \qty{ 1 + {x^2\over n}}^{-(n+1)} \, dx  \\
&= \int_0^\infty e^{-x^2}  \\
&= {\sqrt \pi \over 2}
.\end{align*}

Computing the last integral:

\begin{align*}
\qty{\int_\RR e^{-x^2}\, dx}^2
&= \qty{\int_\RR e^{-x^2}\,dx} \qty{\int_\RR e^{-y^2}\,dx} \\
&= \int_\RR \int_\RR e^{-(x+y)^2}\, dx \\
&= \int_0^{2\pi} \int_0^\infty e^{-r^2} r\, dr \, d\theta \qquad u=r^2 \\
&= {1\over 2} \int_0^{2\pi } \int_0^\infty e^{-u}\, du \, d\theta \\
&= {1\over 2} \int_0^{2\pi} 1 \\
&= \pi
,\end{align*}
and now use the fact that the function is even so $\int_0^\infty f = {1\over 2} \int_\RR f$.

Justifying the DCT:

- ??? (Todo)


## 6 

Concepts used:

- For $e_n(x) \definedas e^{2\pi i n x}$, the set $\theset{e_n}$ is an orthonormal basis for $L^2([0, 1])$.
- For any orthonormal sequence in a Hilbert space, we have Bessel's inequality:
  \begin{align*}
  \sum_{k=1}^{\infty}\left|\left\langle x, e_{k}\right\rangle\right|^{2} \leq\|x\|^{2}
  .\end{align*}
- When $\theset{e_n}$ is a basis, the above is an *equality* (Parseval)
- Arguing uniform convergence: since $\theset{\hat f(n)} \in \ell^1(\ZZ)$, we should be able to apply the $M$ test.

### a

Claim: $\ell^1(\ZZ) \subseteq \ell^2(\ZZ)$.

- Set $\vector c = \theset{c_k \suchthat k\in \ZZ} \in \ell^1(\ZZ)$.
- It suffices to show that if $\sum_{k\in \ZZ} \abs{c_k} < \infty$ then $\sum_{k\in \ZZ} \abs {c_k}^2 < \infty$.
- Let $S = \theset{c_k \suchthat \abs{c_k} \leq 1}$, then $c_k \in S \implies \abs{c_k}^2 \leq \abs{c_k}$
- Claim: $S^c$ can only contain finitely many elements, all of which are finite.
  - If not, either $S^c \definedas \theset{c_j}_{j=1}^\infty$ is infinite with every $\abs{c_j} > 1$, which forces $$\sum_{c_k\in S^c} \abs{c_k} = \sum_{j=1}^\infty \abs{c_j} > \sum_{j=1}^\infty 1 = \infty.$$
  - If any $c_j = \infty$, then $\sum_{k\in \ZZ} \abs{c_k} \geq c_j = \infty$.
- So $S^c$ is a finite set of finite integers, let $N = \max \theset{\abs{c_j}^2 \suchthat c_j \in S^c} < \infty$.
- Rewrite the sum
\begin{align*}
\sum_{k\in \ZZ} \abs{c_k}^2 
&= \sum_{c_k\in S} \abs{c_k}^2 + \sum_{c_k \in S^c} \abs{c_k}^2 \\
&\leq \sum_{c_k\in S} \abs{c_k} + \sum_{c_k \in S^c} \abs{c_k}^2 \\
&\leq \sum_{k\in \ZZ} \abs{c_k} + \sum_{c_k \in S^c} \abs{c_k}^2 \quad\text{since the $\abs{c_k}$ are all positive} \\
&= \norm{\vector c}_{\ell^1} + \sum_{c_k \in S^c} \abs{c_k}^2 \\
&\leq \norm{\vector c}_{\ell^1} + \abs{S^c}\cdot N \\
&< \infty
.\end{align*}

Claim: $L^2([0, 1]) \subseteq L^1([0, 1])$.

- It suffices to show that $\int \abs{f}^2 < \infty \implies \int \abs{f} < \infty$.
- Define $S = \theset{x\in [0, 1] \suchthat \abs{f(x)} \leq 1}$, then $x\in S^c \implies \abs{f(x)}^2 \geq \abs{f(x)}$.

- Break up the integral:
\begin{align*}
\int_\RR \abs f 
&= \int_S \abs f + \int_{S^c} \abs f \\
&\leq \int_S \abs{f} + \int_{S^c} \abs{f}^2 \\
&\leq \int_S \abs{f} + \norm{f}_2 \\
&\leq \sup_{x\in S}\theset{\abs{f(x)}} \cdot \mu(S) + \norm{f}_2 \\
&= 1 \cdot \mu(S) + \norm{f}_2 \quad\text{by definition of } S\\
&\leq 1 \cdot \mu([0, 1]) + \norm{f}_2 \quad\text{since } S\subseteq [0, 1] \\
&= 1 + \norm{f}_2 \\
&< \infty
.\end{align*}


> Note: this proof shows $L^2(X) \subseteq L^1(X)$ whenever $\mu(X) < \infty$.
