# Fall 2016

## 1

- Set $f_N(x) \definedas \sum_{n=1}^N n^{-x}$, so $f(x) = \lim_{N\to\infty} f_N(x)$.
- If an interchange of limits is justified, we have
\[  
\dd{}{x} \lim_{N\to\infty} \sum_{n=1}^N n^{-x}
&= \lim_{N\to\infty} \dd{}{x} \sum_{n=1}^N n^{-x} \\
&= \lim_{N\to\infty} \sum_{n=1}^N \dd{}{x} n^{-x} \quad\text{(since this is a finite sum)}\\
&= \lim_{N\to\infty} \sum_{n=1}^N {-\ln(n) \over n^x}  \\
&= \lim_{N\to\infty} \sum_{n=1}^N {\ln\qty{{1\over n}} \over n^x} 
,\]
  so it suffices to show the last sum converges on $(1, \infty)$.

\todo{No idea how. But if this works, does this show both parts?}

## 2

- If $\int f = \int g$ then $\int \qty{f-g} = 0$, so it suffices to show that $\int f = 0 \implies f = 0$ a.e. or there exists a measurable set $E$ such that $\int_E f > 0$.

- Suppose $\int f = 0$ and it is *not* the case that $f=0$ a.e.
- By definition, if $E\definedas \theset{x\in [a, b] \suchthat f(x) > 0} \neq 0$ then $m(E) > 0$.
- In particular, $f>0$ on $E$, and by monotonicty of the integral, $\int_E f > \int_E 0 = 0$.

## 3

- Fixing notation, set $\tau_x f(y) = f(y-x)$; we then want to show
\[  
\norm{\tau_x f -f}_{L^1} \converges{x\to 0}\to 0
.\]
- By an $\eps/3$ argument, it suffices to show this for compactly supported functions:
  - Since $f\in L^1$, choose $g_n\subset C_c^\infty(\RR^1)$ smooth and compactly supported so that $\norm{f-g_n}_{L^1} \to 0$
  - Then
  \[  
  \norm{\tau_x f - f}_1 
  &= \norm{\tau_x f - \tau_y g_n + \tau_y g_n - g_n +g_n - f}_{1} \\
  &\leq \norm{\tau_y f - \tau_y g_n}_1 + \norm{\tau_y g_n - g_n}_1 + \norm{g_n - f}_{1} \\
  &\leq 2\eps + \norm{\tau_y g_n - g_n}_1
  .\]

- Let $g\in C_c^\infty(\RR^1)$, let $E = \supp(g)$, and write
\[  
\norm{\tau_y g_n - g_n}_1 
&= \int_\RR \abs{g(y-x) - g(y)\,dy \\
&= \int_E g(y)\,dy + \int_{E^c} g(y)\,dy
.\]

