# Fall 2019

## 1

> Cesaro mean/summation. Break series apart into pieces that can be handled separately.

## a

Prove a stronger result: 
$$
a_n \to A \implies \frac 1 N \sum^N a_k \to A
.$$

> Idea: once $N$ is large enough, $a_k \approx A$, and all smaller terms will die off as $N\to \infty$.
>
> See [this MSE answer](https://math.stackexchange.com/questions/514802/convergence-of-series-implies-convergence-of-cesaro-mean).

Suppose $S_k \to S$.
Choose $\ell$ large enough such that 
$$
k\geq \ell \implies \abs{S_k - S} < \varepsilon
.$$

With $\ell$ fixed, choose $N$ large enough such that
$$
k\leq \ell \implies \frac{\left|S_{k}-S\right|}{N} < \varepsilon
.$$

Then
\begin{align*}
\left|\left(\frac{1}{N} \sum_{k=1}^{N} S_{k}\right)-S\right| 
&=\frac{1}{N}\left|\sum_{k=1}^{N}\left(S_{k}-S\right)\right| \\
&\leq \frac{1}{N} \sum_{k=1}^{N}\left|S_{k}-S\right| \\
&= \sum_{k=1}^{\ell}\frac{\left|S_{k}-S\right|}{N} +
\sum_{k=\ell+1}^{N} \frac{\left|S_{k}-S\right|}{N} \\
& \to 0
.\end{align*}

## b

Define
\begin{align*}
\Gamma_n \definedas \sum_{k=n}^\infty \frac{a_k}{k}
.\end{align*}

Then $\Gamma_1 = \sum_k \frac{ a_k } k$ and each $\Gamma_n$ is a tail of this series, so by assumption $\Gamma_n \to 0$.

Then
\begin{align*}
\frac 1 n \sum_{k=1}^n a_k 
&= \frac 1 n (\Gamma_0 + \Gamma_1 + \cdots + \Gamma_{n} \mathbf{- \Gamma_{n+1}}) \\
&\to 0
.\end{align*}

This comes from consider the following summation:

```{=latex}
\begin{tikzcd}
\Gamma_1:&\arrow[dash, ddddd]   & a_1 & + \frac{a_2}{2} & + \frac{a_3}{3} & + \cdots &     &                                    &          &  &  &  \\
\Gamma_2:                                                       &               &     & \frac{a_2}{2}   & + \frac{a_3}{3} & + \cdots &     &                                    &          &  &  &  \\
\Gamma_3:                                                       &               &     &                 & \frac{a_3}{3}   & + \cdots &     &                                    &          &  &  &  \\
 \arrow[dash, rrrrrrrrrr] &&&&&&&&&&{}&   \\
\sum_{i=1}^n \Gamma_i:                                          &               & a_1 & +a_2            & +a_3            & + \cdots & a_n & + \frac{a_{n+1}}{n+1}              & + \cdots &  &  &  \\
& {}               &     &                 &                 &          &     &   &          &  &  & 
\end{tikzcd}
```

$\qed$

## 2

> DCT, and bounding in the right place. Don't evaluate the actual integral!

Use the fact that $\int_0^1 \cos(tx) ~dt = \sin(x)/x$, then
\begin{align*}
\abs {\dd{^n}{x} \sin(x)/x  }
&= \abs { \dd{^n}{x}\int_0^1 \cos(tx)~dt }\\
&=_? \abs{ \int_0^1  \dd{^n}{x} \cos(tx)~dt }\\
&= \abs{ \int_0^1 -t^n \sin(tx) ~dt } \quad \text{for $n$ odd}\\
&\leq \int_0^1 \abs{t^n \sin(tx)} ~dt \\
&\leq \int_0^1 t^n ~dt \\ 
&= \frac{1}{n+1} \\
&< \frac{1}{n}
.\end{align*}

Where the DCT is justified by noting that $f(t) = \cos(tx)$ is dominated by $g(t) = 1$ on $[0, 1]$, which integrates to 1.

$\qed$

## 3

> Borel-Cantelli.
>
> Use the following observation: for a sequence of sets $X_n$, 
>
\begin{align*}
\limsup_n X_n &= \theset{x \suchthat x\in X_n \text{ for infinitely many $n$} } 
&= \intersect_{m\in \NN} \union_{n\geq m} X_n
\\
\liminf_n X_n &= \theset{x \suchthat x\in X_n \text{ for all but finitely many $n$} }
&= \union_{m\in \NN} \intersect_{n\geq m} X_n
.\end{align*}
>
> And recall
>
\begin{align*}
\prod_n e^{x_n} = e^{\sum_n x_n} \quad\text{and} \quad \sum_n \log(x_n) = \log\left(\prod_n x_n\right)
.\end{align*}

### a

The Borel $\sigma\dash$algebra is closed under countable unions/intersections/complements, and $B = \limsup_n B_n$ is an intersection of unions of measurable sets.

### b

We'll use the fact that tails of convergent sums go to zero, so $\sum_{n\geq M} \mu(B_n) \mapsvia{M\to\infty} 0$, and $B_M \definedas \intersect_{m = 1}^M \union_{n\geq m} B_n \searrow B$.

\begin{align*}
\mu(B_M) 
&= \mu\left(\intersect_{m\in \NN} \union_{n\geq m} B_n\right) \\
&\leq \mu\left( \union_{n\geq m} B_n \right) \quad \text{for all } m\in \NN \\
&\to 0
,\end{align*}

and the result follows by continuity of measure.

### c

To show $\mu(B) = 1$, we'll show $\mu(B^c) = 0$.

Let $B_k = \intersect_{m=1}^\infty \union_{n = m}^K B_n$. Then

\begin{align*}
\mu(B_K^c) 
&= \mu \left(\union_{m=1}^\infty \intersect_{n=m}^K B_n^c\right) \\
&\leq \sum_{m=1}^\infty \mu\left( \intersect_{n=m}^K B_n^c \right) \quad\text{ by subadditivity} \\
&= \sum_{m=1}^\infty \prod_{n=m}^K 1 - \mu(B_n) \\
&\leq \sum_{m=1}^\infty \prod_{n=m}^K e^{-\mu(B_n^c)} \quad\text{by hint} \\
&= \sum_{m=1}^\infty e^{-\sum_{n=m}^K \mu(B_n^c)} \\
&\to 0
\end{align*}

since $\displaystyle\sum_{n=m}^K \mu(B_n^c) \to \infty$, and we can apply continuity of measure since $B_K^c \mapsvia{K\to\infty} B^c$.

$\qed$

## 4

> Bessel's Inequality, surjectivity of Riesz map, and Parseval's Identity.
> 
> Trick -- remember to write out finite sum $S_N$, and consider $\norm{x - S_N}$.


### a

**Claim:**
\begin{align*}
0 \leq \left\|x-\sum_{n=1}^{N}\left\langle x, u_{n}\right\rangle u_{n}\right\|^{2}
&= \|x\|^{2}-\sum_{n=1}^{N}\left|\left\langle x, u_{n}\right\rangle\right|^{2} \\ 
&\implies
\sum_{n=1}^{\infty}\left|\left\langle x, u_{n}\right\rangle\right|^{2} \leq\|x\|^{2}
.\end{align*}

*Proof:*
Let $S_N = \sum_{n=1}^N \inner{x}{u_n} u_n$. 
Then
\begin{align*}
0 
&\leq \norm{x - S_N}^2 \\ 
&= \inner{x - S_n}{x - S_N} \\
&= \norm{x}^2 - \sum_{n=1}^N \abs{\inner{x}{u_n}}^2 \\
&\mapsvia{N\to\infty} \norm{x}^2 - \sum_{n=1}^N \abs{\inner{x}{u_n}}^2
.\end{align*}


### b

1. Fix $\theset{a_n} \in \ell^2$, then note that $\sum \abs{a_n}^2 < \infty \implies$ the tails vanish.

2. Define 
$$
x \definedas \displaystyle\lim_{N\to\infty} S_N = \lim_{N\to \infty} \sum_{k=1}^N a_k u_k
$$

3. $\theset{S_N}$ Cauchy (by 1) and $H$ complete $\implies x\in H$.

4.  
$$
\inner{x}{u_n} = \inner{\sum_k a_k u_k}{u_n} = \sum_k a_k \inner{u_k}{u_n} = a_n \quad \forall n\in \NN
$$ 
since the $u_k$ are all orthogonal.

5.
$$
\norm{x}^2 = \norm{\sum_k a_k u_k}^2 = \sum_k \norm{a_k u_k}^2 = \sum_k \abs{a_k}^2
$$ 
by Pythagoras since the $u_k$ are normal.

> Bonus: We didn't use completeness here, so the Fourier series may not actually converge to $x$.
If $\theset{u_n}$ is **complete** (so $x = 0 \iff \inner{x}{u_n} = 0 ~\forall n$) then the Fourier series *does* converge to $x$ and $\sum_{n=1}^{\infty}\left|\left\langle x, u_{n}\right\rangle\right|^{2}=\|x\|^{2}$ for all $x \in H$.

$\qed$

## 5

> Continuity in $L^1$ (recall that DCT won't work! Notes 19.4, prove it for a dense subset first).
>
> Lebesgue differentiation in 1-dimensional case. See HW 5.6.

## a

Choose $g\in C_c^0$ such that $\norm{f- g}_1 \to 0$.

By translation invariance, $\norm{\tau_h f - \tau_h g}_1 \to 0$.

Write
\begin{align*}
\norm{\tau f - f}_1 
&= \norm{\tau_h f - g + g - \tau_h g + \tau_h g - f}_1 \\
&\leq \norm{\tau_h f - \tau_h g} + \norm{g - f} + \norm{\tau_h g - g} \\
&\to \norm{\tau_h g - g}
,\end{align*}

so it suffices to show that $\norm{\tau_h g - g} \to 0$ for $g\in C_c^0$.

Fix $\varepsilon > 0$.
Enlarge the support of $g$ to $K$ such that
\begin{align*}
\abs{h} \leq 1 \text{ and } x \in K^c \implies \abs{g(x-h) - g(x)} = 0
.\end{align*}

By uniform continuity of $g$, pick $\delta \leq 1$ small enough such that 
$$
x\in K, ~\abs{h} \leq \delta \implies \abs{g(x-h) -g(x)} < \varepsilon
,$$

then
$$
\int_K \abs{g(x-h) - g(x)} \leq \int_K \varepsilon = \varepsilon \cdot m(K) \to 0.
$$


## b

We have
\begin{align*}
\int_\RR \abs{A_h(f)(x)} ~dx 
&= \int_\RR \abs{\frac{1}{2h} \int_{x-h}^{x+h} f(y)~dy} ~dx \\
&\leq \frac{1}{2h} \int_\RR \int_{x-h}^{x+h} \abs{f(y)} ~dy ~dx    \\
&=_{FT} \frac{1}{2h} \int_\RR \int_{y-h}^{y+h} \abs{f(y)} ~\mathbf{dx} ~\mathbf{dy}    \\
&= \int_\RR \abs{f(y)} ~{dy} \\
&= \norm{f}_1
.\end{align*}

and (rough sketch)

\begin{align*}
\int_\RR \abs{A_h(f)(x) - f(x)} ~dx 
&= \int_\RR \abs{ \left(\frac{1}{2h} \int_{B(h, x)} f(y)~dy\right) - f(x)}~dx \\
&= \int_\RR \abs{ \left(\frac{1}{2h} \int_{B(h, x)} f(y)~dy\right) - \frac{1}{2h}\int_{B(h, x)} f(x) ~dy}~dx \\
&\leq_{FT} \frac{1}{2h} \int_\RR  \int_{B(h, x)}\abs{ f(y-x) - f(x)} ~\mathbf{dx} ~\mathbf{dy} \\
&\leq \frac 1 {2h} \int_\RR \norm{\tau_x f - f}_1 ~dy \\
&\to 0 \quad\text{by (a)}
.\end{align*}

$\qed$