---
title: Linearization Continued 
subtitle: Section 8.4 Follow-Up 
author: D. Zack Garza
date: April 2020
theme: Berkeley 
colortheme: default 
fontfamily: noto-sans
aspectratio: 169
header-includes:
- \usepackage{cmbright}
fontsize: 10pt
---

[Floer Reading Group Fall 2020](../../../../zets/Floer%20Reading%20Group%20Fall%202020.md)

# Review

## Definitions 

- The Floer equation is given by
  \begin{align*}
  \frac{\partial u}{\partial s}+J(u) \frac{\partial u}{\partial t}+\operatorname{grad} H_{t}(u)=0
  .\end{align*}

- We fixed a solution and lifted it to a sphere:
$$
u \in C^\infty(S^1\cross \RR; W) \quad\mapsto\quad \tilde u \in C^\infty(S^2; W) 
$$ 

- We use the assumption: 
  
  > For every $w\in C^\infty(S^2, W)$ there exists a symplectic trivialization of the fiber bundle $w^* TW$, i.e. $\inner{c_1(TW)}{\pi_2(W)} = 0$ where $c_1$ denotes the first Chern class of the bundle $TW$.

- We use this trivialize the pullback $\tilde u ^* TW$ to obtain an orthonormal unitary frame $$\theset{Z_i}_{i=1}^{2n} \subset T_{u(s, t)} W$$ 

## The Frame 

- We used the chosen frame $\theset{Z_i}$ to define a chart centered at $u$ of $\mcp^{1, p}(x, y)$ given by
\begin{align*}
\iota: W^{1, p}\left(\mathbb{R} \times S^{1} ; \mathbb{R}^{2 n}\right) & \longrightarrow \mathcal{P}^{1, p}(x, y) \\
Y = \left(y_{1}, \dots, y_{2 n}\right) & \longmapsto \exp _{u}\left(\sum y_{i} Z_{i}\right)
.\end{align*}


- We regard $Y(s, t)$ as a tangent vector to $W$ in some Euclidean embedding.


## Charts 

- We seek to compute the composite map in charts:

\begin{center}
\includegraphics[height= 0.5\textheight]{figures/image_2020-04-16-01-11-02.png} 
\end{center}

## Add a Tangent

\begin{center}
\begin{tikzcd}[ampersand replacement=\&, matrix scale=0.002]
\mcf(u) =
\& \frac{\partial u}{\partial s} 
\& + J(u) \frac{\partial u}{\partial t} 
\& - J(u)X_{t}(u) \\
\mathcal{F}(u+Y) =
\& \frac{\partial(u+Y)}{\partial s}
\&+ J(u+Y) \frac{\partial(u+Y)}{\partial t}
\&- J(u+Y) X_{t}(u+Y)
\end{tikzcd}
\end{center}
Extract the part that is linear in $Y$ and collect terms:

\begin{align*}
&(d \mathcal{F})_{u}(Y)  \\
& = {\color{red}\frac{\partial Y}{\partial s}} +(d J)_{u}(Y) \frac{\partial u}{\partial t} + {\color{red} J(u) \frac{\partial Y}{\partial t}} -(d J)_{u}(Y) X_{t}-J(u)\left(d X_{t}\right)_{u}(Y) \\ 
& = 
\qty{ {\color{red}\frac{\partial Y}{\partial s}} + {\color{red} J(u) \frac{\partial Y}{\partial t}}}  \\
& \hspace{2em} + \qty{ (d J)_{u}(Y) \frac{\partial u}{\partial t} - (d J)_{u}(Y) X_{t}-J(u)\left(d X_{t}\right)_{u}(Y)} \\
.\end{align*}


# 8.4.1: Leibniz Rule 


## Leibniz Rule 
Recall the Leibniz rule $$(dJ)(Y) \cdot v = d(Jv)(Y) - J dv(Y)$$
\begin{align*}
(d \mathcal{F})_{u}(Y)
& = 
\qty{ {\color{red}\frac{\partial Y}{\partial s}} + {\color{red} J(u) \frac{\partial Y}{\partial t}}}  \\
& \quad + \qty{ (d J)_{u}(Y) \frac{\partial u}{\partial t} - (d J)_{u}(Y) X_{t}-J(u)\left(d X_{t}\right)_{u}(Y)} \\ 
&= \sum_{i=1}^{2n} \qty{ \dd{y_i}{s} Z_i + \dd{y_i}{t} J(u) Z_i} \\
& + \sum_{i=1}^{2n} y_i \Bigg( \dd{Z_i}{s} + J(u) \dd{Z_i}{t} + (dJ)_u (Z_i) \dd{u}{t}  \\
&\hspace{5em}- J(u) (dX_t)_u Z_i - (dJ)_u (Z_i) X_t \Bigg)
.\end{align*}

Use the fact that this is $O_1 + O_0$ in $Y$.

## Order 1 

Study $O_1$ first, which (claim) reduces to 
  \begin{align*}
  O_1 = \sum_{i=1}^{2n} \qty{\dd{y_i}{s} + J_0 \dd{y_i}{t}  }Z_i = \bar \del(y_1, \cdots, y_{2n})
  .\end{align*}
  where $J_0$ is the standard complex structure on $\RR^{2n} = \CC^n$

Use this to write
\begin{align*}
(d\mcf)_u &= {\color{red} \bar \del Y} + SY
\end{align*}
where $S\in C^\infty(\RR\cross S^1; \endo(\RR^n))$ is a linear operator of order 0.

# Order 0 Part is Symmetric in the Limit

## 8.4.4: Order 0 Part is Symmetric in the Limit
Theorem (8.4.4, CR + Symmetric in the Limit)
:   If $u$ solves Floer's equation, then 
    $$
    (d\mcf)_u = \bar\del + S( s, t)
    $$ 
    where 

    1. $S$ is linear 
    2.  $S$ tends to a symmetric operator as $s\to \pm \infty$, and 
    3. We have the limiting behavior
    $$\dd{S}{s}(s, t)  \converges{s\to\pm\infty}\to 0 \qtext{uniformly in $t$}$$



## Proof

Collect terms in the order zero part:
\begin{align*}
O_0 = S(y_1, \cdots , y_{2n}) 
&= \sum_{i=1}^{2n} y_i \Bigg[ {\color{orange} \dd{Z_i}{s}} + J(u) \dd{Z_i}{t} + {\color{blue} (dJ)_u (Z_i) \dd{u}{t}}  \\
&\hspace{5em}  - J(u) (dX_t)_u Z_i - {\color{blue} (dJ)_u (Z_i) X_t} \Bigg] \\
&= \sum_{i=1}^{2n} y_i \Bigg[ {\color{orange} \dd{Z_i}{s} } + { \color{blue} (dJ)_u (Z_i) \qty{ \dd{u}{t} - (Z_i) X_t} } \\
&\hspace{5em} + {\color{red} J(u) \dd{Z_i}{t}  - J(u) (dX_t)_u Z_i} \Bigg]
.\end{align*}

- Claim: the terms in blue and orange vanish in the limit $s \to \pm \infty$, so it suffices to prove that the red term limits to a symmetric operator.

## Proof: Blue Term Vanishes

$$
{ \color{blue} (dJ)_u (Z_i) \qty{ \dd{u}{t} - (Z_i) X_t} } \to 0
$$

The term in blue vanishes: since $u$ is a solution and 
  
$$\dd{u}{s} \converges{s\to \pm \infty}\to 0 \qtext{uniformly}$$

as do its derivatives, we have

$$ \qty{ \dd{u}{t} - X_t(u)} \converges{s\to \pm\infty}\to 0 $$

> This seems to be the full argument for the blue term.

## Proof: Orange Term Vanishes (1 and 3)

$$
{\color{orange} \dd{Z_i}{s} } \converges{s\to \pm \infty}\to 0 
$$

Follows since the frame $Z_i$ was chosen such that 

$$\dd{}{s}, \quad \frac{\del^2}{\del s^2}, \quad \frac{\del^2}{\del s~\del t} \quad \actson Z_i \converges{s\to \pm\infty}\to 0\quad \text{for each } i$$

This also implies

$$ \dd{S}{s} \converges{s\to \pm\infty}\to 0.$$

> This shows parts (1) and (3) of the theorem: linearity and limits to zero uniformly in $t$?

## Proof: Symmetry

Write the remaining red term as 

\begin{align*}
A \definedas A\left(y_{1}, \ldots, y_{2 n}\right)=\sum y_{i}\left( {\color{red} J(u) \frac{\partial Z_{i}}{\partial t}-J(u)\left(d X_{t}\right)_{u}\left(Z_{i}\right) } \right)
.\end{align*}


Extract the $j$th component:
\begin{align*}
A_j = \sum y_{i}\left\langle J(u) \frac{\partial Z_{i}}{\partial t}-J(u)\left(d X_{t}\right)_{u}\left(Z_{i}\right), \quad Z_{j}\right\rangle
.\end{align*}

We'll show that
\begin{align*}
\lim _{s \rightarrow \pm \infty}
&\left\langle J(u) \frac{\partial Z_{\color{red} i}}{\partial t}-J(u)\left(d X_{t}\right)_{u}\left(Z_{\color{red} i}\right), Z_{\color{red} j}\right\rangle \\
- &\left\langle J(u) \frac{\partial Z_{\color{red} j}}{\partial t}-J(u)\left(d X_{t}\right)_{u} Z_{\color{red}j}, ~~~Z_{\color{red} i}\right\rangle=0
.\end{align*}

## Proof: Symmetry

Use the fact that the frame $\theset{Z_i}$ is unitary:
\begin{align*}
0 &=\frac{\partial}{\partial t}\left\langle J(u) Z_{i}, Z_{j}\right\rangle \\
&=\left\langle(d J)_{u}\left(\frac{\partial u}{\partial t}\right) Z_{i}, Z_{j}\right\rangle+\left\langle J(u) \frac{\partial Z_{i}}{\partial t}, Z_{j}\right\rangle+\left\langle {\color{red} J(u) } Z_{i}, \frac{\partial Z_{j}}{\partial t}\right\rangle \\
&=
\left\langle(d J)_{u}\left(\frac{\partial u}{\partial t}\right) Z_{i}, Z_{j}\right\rangle+\left\langle J(u) \frac{\partial Z_{i}}{\partial t}, Z_{j}\right\rangle-\left\langle Z_{i}, {\color{red} J(u)} \frac{\partial Z_{j}}{\partial t}\right\rangle
.\end{align*}

## Proof: Symmetry

Therefore it suffices to show
\begin{align*}
-&\left\langle J(u)\left(d X_{t}\right)_{u}\left(Z_{i}\right), \quad Z_{j}\right\rangle \\
+&\left\langle J(u)\left(d X_{t}\right)_{u}\left(Z_{j}\right), \quad Z_{i}\right\rangle \\
-&\left\langle(d J)_{u}\left(\frac{\partial u}{\partial t}\right) Z_{i}, \quad Z_{j}\right\rangle \\ \\
&\converges{s\to \pm\infty}\to 0
.\end{align*}

## Proof: Symmetry

Using the fact that
\begin{align*}
\qty{ \dd{u}{t} - X_t(u)} \converges{s\to \pm\infty}\to 0
\end{align*}

we can equivalently show
\begin{align*}
&- \left\langle J(u)\left(d X_{t}\right)_{u}\left(Z_{i}\right), \quad Z_{j}\right\rangle \\
&+ \left\langle J(u)\left(d X_{t}\right)_{u} \left(Z_{j}\right), \quad Z_{i}\right\rangle \\
&- \left\langle(d J)_{u}\left(X_{t}\right) Z_{i}, \hspace{2.5em} Z_{j}\right\rangle \\ \\
&\converges{s\to \pm\infty}\to 0
\end{align*}

> For a fixed $(s, t)$, this expression only depends on $Z_i$ at the point $u(s, t)$.


# Lemma That Concludes the Proof

## Lemma

**Lemma**: For $p\in W$, $\theset{Z_i}$ a unitary basis of $T_p W$, 
\begin{align*}
&- \left\langle J(p)\left(d X_{t}\right)_{p}\left(Z_{i}\right), \quad Z_{j}\right\rangle \\
&+ \left\langle J(p)\left(d X_{t}\right)_{p}\left(Z_{j}\right), \quad Z_{i}\right\rangle \\
&- \left\langle(d J)_{p}\left(X_{t}\right) Z_{i}, \hspace{2.5em} Z_{j}\right\rangle \\
&= 0
.\end{align*}

**Claim**:
This lemma immediately concludes the previous proof?

## Proof of Lemma

Extend $\theset{Z_i}$ to a chart containing $p$ and use the Leibniz rule to rewrite

\small
\begin{align*}
- \left\langle J(p)\left(d X_{t}\right)_{p}\left(Z_{i}\right), Z_{j}\right\rangle 
+ \left\langle J(p)\left(d X_{t}\right)_{p}\left(Z_{j}\right), Z_{i}\right\rangle 
- \left\langle(d J)_{p}\left(X_{t}\right) Z_{i}, Z_{j}\right\rangle 
= 0
\end{align*}
\normalsize
as
\footnotesize
\begin{align*}
&- \left\langle J\left(d X_{t}\right)\left(Z_{i}\right),Z_{j}\right\rangle 
+ \left\langle J\left(d X_{t}\right)\left(Z_{j}\right), Z_{i}\right\rangle
+ \left\langle J\left(d Z_{i}\right)\left(X_{t}\right), Z_{j}\right\rangle  
- {\color{red} \left\langle d\left(J Z_{i}\right)\left(X_{t}\right), Z_{j}\right\rangle } \\ \\
&=\left\langle J\left[X_{t}, Z_{i}\right], Z_{j}\right\rangle 
+ \left\langle J\left(d X_{t}\right)\left(Z_{j}\right), Z_{i}\right\rangle 
- {\color{red} \left\langle d\left(J Z_{i}\right)\left(X_{t}\right), Z_{j}\right\rangle }
.\end{align*}
\normalsize

where we'll rewrite the red terms.

## Proof of Lemma

\scriptsize

Now use
\begin{align*}
X_t \inner{JZ_i}{Z_j} = 0 
\implies
\left\langle d\left(J Z_{i}\right)\left(X_{t}\right), Z_{j}\right\rangle+\left\langle J Z_{i},\left(d Z_{j}\right)\left(X_{t}\right)\right\rangle=0
.\end{align*}

We now rewrite the RHS from before:
\begin{align*}
\left\langle J\left[X_{t}, Z_{i}\right], Z_{j}\right\rangle &+\left\langle J\left(d X_{t}\right)\left(Z_{j}\right), Z_{i}\right\rangle+\left\langle J Z_{i},\left(d Z_{j}\right)\left(X_{t}\right)\right\rangle \\ \\
&=\left\langle J\left[X_{t}, Z_{i}\right], Z_{j}\right\rangle+\left\langle J\left(d X_{t}\right)\left(Z_{j}\right)-J\left(d Z_{j}\right)\left(X_{t}\right), Z_{i}\right\rangle \\
&=\left\langle J\left[X_{t}, Z_{i}\right], Z_{j}\right\rangle-\left\langle J\left[X_{t}, Z_{j}\right], Z_{i}\right\rangle \\
&=\omega\left(\left[X_{t}, Z_{i}\right], Z_{j}\right)-\omega\left(\left[X_{t}, Z_{j}\right], Z_{i}\right)
.\end{align*}

The symmetry follows from $\omega$ being closed and
\begin{align*}
0
&= d \omega\left(X_{t}, Z_{i}, Z_{j}\right) \\
&= X_{t} \cdot \omega\left(Z_{i}, Z_{j}\right)-Z_{i} \cdot \omega\left(X_{t}, Z_{j}\right)+Z_{j} \cdot \omega\left(X_{t}, Z_{i}\right) \\
&\quad -\omega\left(\left[X_{t}, Z_{i}\right], Z_{j}\right)+\omega\left(\left[X_{t}, Z_{j}\right], Z_{i}\right)-\omega\left(\left[Z_{i}, Z_{j}\right], X_{t}\right) \\ \\
&= -X_{t} \cdot\left\langle Z_{i}, J Z_{j}\right\rangle+Z_{i} \cdot\left(d H_{t}\right)\left(Z_{j}\right)-Z_{j} \cdot\left(d H_{t}\right)\left(Z_{i}\right) \\
&\quad -\left(d H_{t}\right)\left(\left[Z_{i}, Z_{j}\right]\right)-\omega\left(\left[X_{t}, Z_{i}\right], Z_{j}\right)+\omega\left(\left[X_{t}, Z_{j}\right], Z_{i}\right) \\ \\
&= d\left(d H_{t}\right)\left(Z_{i}, Z_{j}\right)-\omega\left(\left[X_{t}, Z_{i}\right], Z_{j}\right)+\omega\left(\left[X_{t}, Z_{j}\right], Z_{i}\right) \\
&= -\omega\left(\left[X_{t}, Z_{i}\right], Z_{j}\right)+\omega\left(\left[X_{t}, Z_{j}\right], Z_{i}\right). \hspace{9em} \qed
\end{align*}

# 8.4.6: Linearization of Hamilton's Equation 

## Linearization of Hamilton's Equation 

Recall
$$
\qty{d\mcf}_u = \bar \del Y + SY = \qty{\bar \del + S}Y 
$$

Now think of $S$ as a map $Y \mapsto S\cdot Y$, so $S\in C^\infty(\RR\cross S^1; \endo(\RR^{2n}))$ and define the symmetric operators
$$
S^{\pm} \definedas  \lim_{s\to \pm\infty} S(s, \wait) \qtext{respectively}
$$

Theorem
:   The equation 
    $$
    \del_t Y = J_0 S^{\pm} Y
    $$ 
    is a linearization of Hamilton's equation 
    \begin{align*}
    \dd{z}{t} = X_t(z)\qtext{at} 
    \begin{cases}
    x = \lim_{s\to -\infty} u & \text{for } S^- \\
    y = \lim_{s\to \infty} u & \text{for } S^+
    \end{cases}\quad\text{respectively}
    .\end{align*}


## Proof

We first linearize Hamilton's equation at $x$:
\begin{align*}
\dd{z}{t} = X_t(z) \quad \stackrel{\text{linearized}}\implies \quad \dd{Y}{t} = (dX_t)_x Y
.\end{align*}

So write $Y = \sum y_i Z_i$ to obtain
\begin{align*}
\sum_{i} \frac{\partial y_{i}}{\partial t} Z_{i} &=\sum_{i} y_{i}\left(-\frac{\partial Z_{i}}{\partial t}+\left(d X_{t}\right)\left(Z_{i}\right)\right) \\
&=\sum_{i} \sum_{j} y_{i}\left\langle-\frac{\partial Z_{i}}{\partial t}+\left(d X_{t}\right)\left(Z_{i}\right), Z_{j}\right\rangle Z_{j} \\
&=\sum_{i} \sum_{j} y_{j}\left\langle-\frac{\partial Z_{i}}{\partial t}+\left(d X_{t}\right)\left(Z_{j}\right), Z_{i}\right\rangle Z_{i} \\ \\
\implies
\frac{\partial y_{i}}{\partial t}
&=\sum_{j}\left\langle-\frac{\partial Z_{j}}{\partial t}+\left(d X_{t}\right)\left(Z_{j}\right), Z_{i}\right\rangle y_{j}
.\end{align*}

## Proof

Thus we can rewrite the linearized equation as
\scriptsize
\begin{align*}
\dd{Y}{t} = (dX_t)_x Y = B^- \cdot Y, \quad 
b_{i j}=\left\langle-\frac{\partial Z_{j}}{\partial t}+\left(d X_{t}\right)_{x}\left(Z_{j}\right), Z_{i}\right\rangle
.\end{align*}
\normalsize 

Recall
\scriptsize
\begin{align*}
A \definedas A\left(y_{1}, \ldots, y_{2 n}\right)=\sum y_{i}\left( {\color{red} J(u) \frac{\partial Z_{i}}{\partial t}-J(u)\left(d X_{t}\right)_{u}\left(Z_{i}\right) } \right)
.\end{align*}
\normalsize

Now take $s\to -\infty$ and look at the order zero part of $(d\mcf)_u$.
By the proof of 8.4.4, we have
\scriptsize
\begin{align*}
A\left(\sum y_{i} Z_{i}\right) &=\sum_{i}\left(J(x) \frac{\partial Z_{i}}{\partial t}-J(x)\left(d X_{t}\right)_{x}\left(Z_{i}\right)\right) \\
&=\sum_{i} \sum_{j} y_{i}\left\langle J \frac{\partial Z_{i}}{\partial t}-J\left(d X_{t}\right)\left(Z_{i}\right), Z_{j}\right\rangle Z_{j} \\
&=\sum_{i} \sum_{j} y_{j}\left\langle J \frac{\partial Z_{j}}{\partial t}-J\left(d X_{t}\right)\left(Z_{j}\right), Z_{i}\right\rangle Z_{i} \\
&=\sum_{i} \sum_{j}\left\langle-\frac{\partial Z_{j}}{\partial t}+\left(d X_{t}\right)\left(Z_{j}\right), J Z_{i}\right\rangle {y_{j}} Z_{i}
.\end{align*}
\normalsize

## Proof

Deduce that 
\begin{align*}
S = (s_{ij}),\quad & s_{ij} = \left\langle-\frac{\partial Z_{j}}{\partial t}+\left(d X_{t}\right)_{x}\left(Z_{j}\right), ~~J(x) Z_{i}\right\rangle \\ \\ \\
JZ_i = \begin{cases}
Z_{i+n} & i \leq n \\
-Z_{i-n} & i \geq n+1
\end{cases}
&\implies 
s_{ij} = 
\begin{cases}
b_{i+n, j} & i \leq n \\
-b_{i-n, j} & i \geq n+1
\end{cases} \\ \\
&\iff S^- = - J_0 B^- 
.\end{align*}
$\qed$
