# Fall 2019

## 1

> Centralizer: 
$$
C_G(h) = Z(h) = \theset{g\in G \suchthat [g,h] = 1}
\quad\text{Centralizer}
$$
>
> Class equation: 
$$
\abs{G} = \sum_{\substack{\text{One $h$ from each } \\ \text{ conjugacy class}}} \frac{\abs{G}}{\abs{Z(h)}}
$$
> Notation:
> \begin{align*}
h^g &= ghg\inv \\
h^G &= \theset{ h^g \suchthat g\in G} \quad\text{Conjugacy Class}\\
H^g &= \theset{h^g \suchthat h\in H} \\
N_G(H) &= \theset{g\in G \suchthat H^g = H} \supseteq H \quad\text{Normalizer}
.\end{align*}
>
> **Theorem 1**: $\abs{h^G} = [G: Z(h)]$
> 
> **Theorem 2**: $\abs{\theset{H^g \suchthat g\in G}} = [G: N_G(H)]$
>
> *Proof:* Let $G\actson \theset{H \suchthat H \leq G}$ by $H \mapsto gHg\inv$.
> Then the $\mathcal O_H$ is the set of conjugate subgroups, $\mathrm{Stab}(H) = N_G(H)$.
> So Orbit-Stabilizer says $\mathcal O_h \cong G/\mathrm{Stab}(H)$; then just take sizes.

> **Theorem 3:** $\union_{g\in G} H^g = \union_{g\in G} gHg\inv \subsetneq G$ for any proper $H \leq G$.
>
> *Proof:* By theorem 2, since each coset is of size $\abs{H}$, which only intersect at the identity, and there are exactly $[G: N_G(H)]$ of them
\begin{align*}
\abs{\union_{g\in G} H^g} 
&= \qty{ \abs{H} - 1} [G: N_G(H)] + 1\\
&= \abs{H} [G: N_G(H)]  - [G:N_G(H)] + 1\\
&= \abs{G} \frac{\abs G}{\abs{N_G(H)}} - \frac{\abs G}{\abs{N_G(H)}} + 1 \\
&\leq \abs{H} \frac{\abs G}{\abs{H}} - \frac{\abs G}{\abs{H}} + 1 \\
&= \abs{G} - ([G: H] - 1) \\
&< \abs{G} 
.\end{align*}
> where we use the fact that $H \subseteq N_G(H) \implies \abs{H} \leq \abs{N_G(H)} \implies \frac{1}{\abs{N_G(H)}} \leq \frac{1}{\abs{H}}$, and since $H < G$ is proper, $[G:H] \geq 2$.

Since $[g_i, g_j] = 1$, we have $g_i \in Z(g_j)$ for every $i, j$.

Then
\begin{align*}
g\in G 
&\implies g = g_i^h \quad \text{ for some } h \\
&\implies g \in Z(g_\mathbf{j})^h \quad\text{for every } j \text{ since }g_i \in Z(g_j) ~\forall j \\
&\implies g \in \union_{h\in G} Z(g_j)^h \quad\text{for every } j\\
&\implies G \subseteq \union_{h\in G} Z(g_j)^h \quad\text{for every } j
,\end{align*}

which by Theorem 3, if $Z(g_j) < G$ were proper, then the RHS is properly contained in $G$. 
So it must be the case that that $Z(g_j)$ is not proper and thus equal to $G$ for every $j$.

But $Z(g_i) = G \iff g_i \in Z(G)$, and so each conjugacy class is size one.
So for every $g\in G$, we have $g = g_j$ for some $j$, and thus $g = g_j \in Z(g_j) = Z(G)$, so $g$ is central.
Then $G\subseteq Z(G)$ and $G$ is abelian.


## 2

> $pqr$ Theorem.

### a

> Recall $n_p \divides m$ and $n_p \cong 1 \mod p$.

An easy check:
\begin{align*}
n_3 \in \theset{1, 7} \quad n_5 \in \theset{1, 21} \quad n_7 \in \theset{1, 15}
.\end{align*}

Toward a contradiction, if $n_5\neq 1$ and $n_7 \neq 1$, then $Q, R$ contribute
\begin{align*}
(5-1)n_5 + (7-1)n_7 + 1 
&= 4(21) + 6(15) > 105 \text{ elements}
.\end{align*}

### b

> If $H, K \leq G$ and $H\normal G$ then $HK \leq G$ is a subgroup.
> Proof: Check closure under products, needs normality.
> 
> **Theorem**: For a positive integer $n$, all groups of order $n$ are cyclic $\iff n$ is
squarefree and, for each pair of distinct primes $p$ and $q$ dividing $n$, $q - 1 \neq 0 \mod p$.
>
> Theorem: If $G = A_1 A_2 \cdots A_n = \prod A_k$ and $A_i \intersect \prod_{k\neq i}A_i = \theset{e}$ for all $i$, then $A \cong A_1 \cross \cdots \cross A_n$.

Either $Q$ or $R$ is normal, so $QR \leq G$ is a subgroup of order $\abs{Q} \cdot \abs{R} = 5\cdot 7 = 35$.

By the theorem, since $5 \notdivides 7-1$, $QR$ is cyclic.

### c

In $QR$, there are 

- $35 - 5 + 1$ elements of order *not* equal to 5,
- $5 - 7 + 1$ elements of order *not* equal to 7.

Since $QR \leq G$, there are *at least* this many such elements in $G$.

Suppose $n_5 = 21$ or $n_7 = 15$.

- Combining elements of order 5 with elements *not* of order 5 yields at least 31 elements of order *not* 5 with $n_5(5-1) = 21(4) = 84$ elements of order 5, this contributes $31 + 84 > 105$ elements -- contradiction.

- Similarly, there are at least $29$ elements of order *not* 7, plus $n_7(7-1) = 15(6) = 90$ elements of order 7, yielding $29 + 90 > 105$ elements.

So both $n_5=1, n_7 = 1$.

### d
If $P$ is normal, then $G=PQR$ with all intersections of the form $AB\intersect C = \theset{e}$, and since $P,Q,R$ are all normal we have $G \cong P\times Q \times R \cong \ZZ_3 \times \ZZ_5 \times \ZZ_7 \cong \ZZ_{105}$ by characterization of direct products and the Chinese Remainder theorem (which is cyclic).


## 3

> Just fiddling with computations.
> Context hints that we should be considering things like $x^2$ and $a+b$.

### a
\begin{align*}
2a  = (2a)^2 = 4a^2 = 4a \implies 2a = 0
.\end{align*}

Note that this implies $x = -x$ for all $x\in R$.

### b
\begin{align*}
a+b = (a+b)^2 &= a^2 + ab + ba + b^2 = a + ab + ba + b \\
&\implies ab + ba = 0 \\
&\implies ab = -ba \\
&\implies ab = ba \quad\text{by (a)}
.\end{align*}

## 4

> Theorem: $F\units$ is always cyclic for $F$ a field

### a

Since $\abs{F} = q$ and $[E:F] = k$, we have $\abs{E} = q^k$ and $\abs{E\units} = q^k-1$.
Noting that $\zeta \in E\units$ we must have $n = o(\zeta) \divides \abs{E\units} = q^k-1$ by Lagrange's theorem.

### b

Rephrasing (a), we have 
\begin{align*}
n \divides q^k-1 
&\iff q^k-1 \cong 0 \mod n \\
&\iff q^k \cong 1 \mod n \\
&\iff m \definedas o(q) \divides k
.\end{align*}

### c

Since $m\divides k \iff k = \ell m$, (**claim**) there is an intermediate subfield $M$ such that
\begin{align*}
E \leq M \leq F \quad k = [F:E] = [F:M] [M:E] = \ell m
,\end{align*}

so $M$ is a degree $m$ extension of $E$.

Now consider $M\units$. 
By the argument in (a), $n$ divides $q^m - 1 = \abs{M\units}$, and $M\units$ is cyclic, so it contains a cyclic subgroup $H$ of order $n$.

But then $x\in H \implies p(x)\definedas x^n-1 = 0$, and since $p(x)$ has at most $n$ roots in a field. 
So $H = \theset{x \in M \suchthat x^n-1 = 0}$, i.e. $H$ contains all solutions to $x^n-1$ in $E[x]$.

But $\zeta$ is one such solution, so $\zeta \in H \subset M\units \subset M$.
Since $F[\zeta]$ is the smallest field extension containing $\zeta$, we must have $F = M$, so $\ell = 1$, and $k = m$.

> Todo: **revisit**, tricky!

## 5

> One-step submodule test.

### a

It suffices to show that 
$$
r\in R, ~t_1, t_2\in \Tor(M) \implies rt_1 + t_2 \in \Tor(M)
.$$

We have
\begin{align*}
t_1 \in \Tor(M) &\implies \exists s_1 \neq 0 \text{ such that } s_1 t_1  = 0 \\
t_2 \in \Tor(M) &\implies \exists s_2 \neq 0 \text{ such that } s_2 t_2  = 0 
.\end{align*}

Since $R$ is an integral domain, $s_1 s_2 \neq 0$.
Then
\begin{align*}
s_1 s_2(rt_1 + t_2) 
&= s_1 s_2 r t_1 + s_1 s_2t_2 \\
&= s_2 r (s_1 t_1) + s_1 (s_2 t_2)  \quad\text{since $R$ is commutative} \\
&=  s_2 r(0) + s_1(0) \\
&= 0
.\end{align*}

### b

Let $R = \ZZ/6\ZZ$ as a $\ZZ/6\ZZ \dash$module, which is not an integral domain as a ring.

Then $[3]_6\actson [2]_6 = [0]_6$ and $[2]_6\actson [3]_6 = [0]_6$, but $[2]_6 + [3]_6 = [5]_6$, where 5 is coprime to 6, and thus $[n]_6\actson [5]_6 = [0] \implies [n]_6 = [0]_6$. So $[5]_6$ is *not* a torsion element.

So the set of torsion elements are not closed under addition, and thus not a submodule.

### c

Suppose $R$ has zero divisors $a,b \neq 0$ where $ab = 0$.
Then for any $m\in M$, we have $b\actson m \definedas bm \in M$ as well, but then 
$$
a\actson bm = (ab)\actson m = 0\actson m = 0_M
,$$ 
so $m$ is a torsion element for any $m$.

$\qed$

## 6

> Prime ideal: $\mathfrak{p}$ is prime iff $ab \in \mathfrak{p} \implies a\in \mathfrak{p}$ or $b\in \mathfrak{p}$.
> Silly fact: 0 is in every ideal!
> 
> **Zorn's Lemma:** Given a poset, if every chain has an upper bound, then there is a maximal element. (Chain: totally ordered subset.)
> 
> **Corollary:** If $S\subset R$ is multiplicatively closed with $0\not\in S$ then $\theset{I \normal R \suchthat J\intersect S = \emptyset}$ has a maximal element.
> (TODO: PROVE)
>
> **Theorem:** If $R$ is commutative, maximal $\implies$ prime for ideals.
> (TODO: PROVE)
>
> **Theorem:** Non-units are contained in a maximal ideal. (See HW?)

### a

Let $\mathfrak{p}$ be prime and $x\in N$.
Then $x^k = 0 \in \mathfrak{p}$ for some $k$, and thus $x^k = x x^{k-1} \in \mathfrak p$.
Since $\mathfrak p$ is prime, inductively we obtain $x\in\mathfrak p$.

### b

Let $S = \theset{r^k \mid k\in \NN}$ be the set of positive powers of $r$. 
Then $S^2 \subseteq S$, since $r^{k_1}r^{k_2} = r^{k_1+k_2}$ is also a positive power of $r$, and $0\not\in S$ since $r\neq 0$ and $r\not\in N$.

By the corollary, $\theset{I \normal R \suchthat I\intersect S = \emptyset}$ has a maximal element $\mathfrak{p}$.

Since $R$ is commutative, $\mathfrak{p}$ is prime.

### c

Suppose $R$ has a unique prime ideal $\mathfrak{p}$.

Suppose $r\in R$ is not a unit, and toward a contradiction, suppose that $r$ is also not nilpotent.

Since $r$ is not a unit, $r$ is contained in some maximal (and thus prime) ideal, and thus $r \in \mathfrak{p}$.

Since $r\not\in N$, by (b) there is a maximal ideal $\mathfrak{m}$ that avoids all positive powers of $r$. 
Since $\mathfrak{m}$ is prime, we must have $\mathfrak{m} = \mathfrak{p}$.
But then $r\not\in \mathfrak{p}$, a contradiction.

## 7

> Galois Theory.
> 
> **Galois** = normal + separable.
> 
> **Separable**: Minimal polynomial of every element has distinct roots.
> 
> **Normal (if separable)**: Splitting field of an irreducible polynomial.

> Definition: $\zeta$ is a primitive root of unity iff $o(\zeta) = n$ in $F\units$.
> 
> $\phi(p^k) = p^{k-1}(p-1)$

> The lattice: 

![](2019-12-24-13-19-15.png)

Let $K = \QQ(\zeta)$. 
Then $K$ is the splitting field of $f(x) = x^n - 1$, which is irreducible over $\QQ$, so $K/\QQ$ is normal.
We also have $f'(x) = nx^{n-1}$ and $\gcd(f, f') = 1$ since they can not share any roots.

> Or equivalently, $f$ splits into distinct linear factors $f(x) = \prod_{k\leq n}(x-\zeta^k)$.

Since it is a Galois extension, $\abs{\Gal(K/\QQ)} = [K: \QQ] = \phi(n)$ for the totient function.

We can now define maps
\begin{align*}
\tau_j: K &\to K \\
\zeta &\mapsto \zeta^j 
\end{align*}

and if we restrict to $j$ such that $\gcd(n, j) = 1$, this yields $\phi(n)$ maps.
Noting that if $\zeta$ is a primitive root, then $(n, j) = 1$ implies that that $\zeta^j$ is also a primitive root, and hence another root of $\min(\zeta, \QQ)$, and so these are in fact automorphisms of $K$ that fix $\QQ$ and thus elements of $\Gal(K/\QQ)$.

So define a map
\begin{align*}
\theta: \ZZ_n\units &\to K \\
[j]_n &\mapsto \tau_j
.\end{align*}

from the *multiplicative* group of units to the Galois group.

The claim is that this is a surjective homomorphism, and since both groups are the same size, an isomorphism.

**Surjectivity:**

Letting $\sigma \in K$ be arbitrary, noting that $[K: \QQ]$ has a basis $\theset{1, \zeta, \zeta^2, \cdots, \zeta^{n-1}}$, it suffices to specify $\sigma(\zeta)$ to fully determine the automorphism.
(Since $\sigma(\zeta^k) = \sigma(\zeta)^k$.)

In particular, $\sigma(\zeta)$ satisfies the polynomial $x^n - 1$, since $\sigma(\zeta)^n = \sigma(\zeta^n) = \sigma(1) = 1$, which means $\sigma(\zeta)$ is another root of unity and $\sigma(\zeta) = \zeta^k$ for some $1\leq k \leq n$.

Moreover, since $o(\zeta) = n \in K\units$, we must have $o(\zeta^k) = n \in K\units$ as well. Noting that $\theset{\zeta^i}$ forms a cyclic subgroup $H\leq K\units$, then $o(\zeta^k) = n \iff (n, k) = 1$ (by general theory of cyclic groups).

Thus $\theta$ is surjective.

**Homomorphism:**

\begin{align*}
\tau_j \circ \tau_k (\zeta) =\tau_j(\zeta^k) = \zeta^{jk} \implies
\tau_{jk} = \theta(jk) = \tau_j \circ \tau_k
.\end{align*}

**Part 2:**

We have $K \cong \ZZ_{20}\units$ and $\phi(20) = 8$, so $K \cong \ZZ_8$, so we have the following subgroups and corresponding intermediate fields:

- $0 \sim \QQ(\zeta_{20})$
- $\ZZ_2 \sim \QQ(\omega_1)$
- $\ZZ_4 \sim \QQ(\omega_2)$
- $\ZZ_8 \sim \QQ$

For some elements $\omega_i$ which exist by the primitive element theorem.


## 8

### a.

Let $\vector v \in \Lambda$, so $\vector v = \sum r_i \vector e_i$ where $r_i \in \ZZ$.

Then if $\vector x = \sum s_i \vector e_i \in \Lambda$, we have
\begin{align*}
\vector v \cdot \vector x = \sum r_i s_i \in \ZZ
\end{align*}

since each term is just a product of integers, so $\vector v \in \Lambda\dual$ by definition.

### b. 


**$\det M \neq 0$**:

Suppose $\det M = 0$. Then $\ker M \neq \vector 0$, so let $\vector v \in \ker M$ be given by $\vector v = [v_1, \cdots, v_n]$.

Note that 
\begin{align*}
M\vector v = 0 &\implies
\left[
\begin{array}{ccc}
\vector e_1 \cdot \vector e_1 & \vector e_1 \cdot \vector e_2 & \cdots \\
\vector e_2 \cdot \vector e_1 & \vector e_2 \cdot \vector e_2 & \cdots \\
\vdots & \vdots & \ddots
\end{array}
\right]
\left[\begin{array}{c}
v_1 \\ v_2 \\ \vdots
\end{array}\right] = \vector 0 \\ \\
&\implies \sum_j (\vector e_1 \cdot  \vector e_j) v_j = 0 \quad \forall j
.\end{align*}

Let $\vector w = \sum v_i \vector e_i$. 
Then $\vector e_k \cdot \vector w = \sum_j v_j \vector e_k \cdot \vector e_j = 0$ for every $k$, so $\vector w$ is orthogonal to every $\vector e_k$, and thus its span.

But $\vector w$ is in the span of the $\vector e_i$ by definition, so 
$$
\vector w \cdot \vector w = 0 \implies \vector w = 0 \implies\theset{\vector e_i} \text{ is linearly dependent}
,$$ 
a contradiction.

$\qed$

*Alternative proof:*

Write $M = A^tA$ where $A$ has the $\vector e_i$ as columns. Then
\begin{align*}
M\vector x = 0 
&\implies A^t A \vector x = 0 \\
&\implies \vector x^t A^t A \vector x = 0 \\
&\implies \norm{A \vector x}^2  = 0 \\
&\implies A\vector x = 0 \\
&\implies \vector x = 0
,\end{align*}

since $A$ has full rank because the $\vector e_i$ are linearly independent.

$\qed$

**The rows of $M\inv$ span $\Lambda\dual$**:

Equivalently, the columns of $M^{-t}$ span $\Lambda\dual$.

> Possibly an error -- should be the rows of $A\inv$ instead of $M\inv$?

Let $B = A^{-t}$ and let $\vector b_i$ denote the columns of $B$, i.e. the span of $\im B$.


Since $A \in \GL(n, \ZZ)$ which is a group, $A\inv, A^t, A^{-t} \in \GL(n, \ZZ)$ as well.

\begin{align*}
\vector v \in \Lambda\dual 
&\implies \vector e_i \cdot \vector v = z_i \in \ZZ \quad \forall i \\
&\implies A^t \vector v = \vector z \in \ZZ^n \\
&\implies \vector v = A^{-t} \vector z \definedas B\vector z \in \im B \\
&\implies \spanof~\Lambda\dual \subseteq \im B
,\end{align*}

and

\begin{align*}
B^t A = (A^{-t})^t A = A\inv A = I \\
\implies \vector b_i \cdot \vector e_j = \delta_{ij} \in \ZZ \\
\implies \im B \subseteq \spanof~ \Lambda\dual
.\end{align*}

$\qed$

### c.

?
